@prefix dcterms: <http://purl.org/dc/terms/> .
@prefix linkml: <https://w3id.org/linkml/> .
@prefix owl: <http://www.w3.org/2002/07/owl#> .
@prefix rdfs: <http://www.w3.org/2000/01/rdf-schema#> .
@prefix skos: <http://www.w3.org/2004/02/skos/core#> .
@prefix xsd: <http://www.w3.org/2001/XMLSchema#> .

<https://example.org/ccdh> a owl:Ontology ;
    rdfs:label "CRDC-H" ;
    dcterms:license "https://creativecommons.org/publicdomain/zero/1.0/" ;
    skos:editorialNote "Derived from [CDM_Dictionary_v1 (Active)](https://docs.google.com/spreadsheets/d/1oWS7cao-fgz2MKWtyr8h2dEL9unX__0bJrWKv6mQmM4)" ;
    linkml:generation_date "2021-05-27 11:48" ;
    linkml:metamodel_version "1.7.0" ;
    linkml:source_file "ccdhmodel.yaml" ;
    linkml:source_file_date "Thu May 27 11:47:18 2021" ;
    linkml:source_file_size 522298 .

<https://example.org/ccdh/CancerGradeObservation> a owl:Class,
        linkml:ClassDefinition ;
    rdfs:label "CancerGradeObservation" ;
    rdfs:subClassOf [ a owl:Restriction ;
            owl:onClass <http://UNKNOWN.org/enum_CRDC-H.CancerGradeObservation.observation_type> ;
            owl:onProperty linkml:observation_type ;
            owl:qualifiedCardinality 1 ],
        [ a owl:Restriction ;
            owl:maxQualifiedCardinality 1 ;
            owl:onClass <http://UNKNOWN.org/enum_CRDC-H.CancerGradeObservation.valueCodeableConcept> ;
            owl:onProperty linkml:valueCodeableConcept ],
        <https://example.org/ccdh/Entity> ;
    skos:definition "A data structure with key (observation_type) and value (valueCodeableConcept) attributes that represents a single cancer grade observation, such as ..." ;
    skos:editorialNote "Derived from [CancerGradeObservation in sheet CancerGrade](https://docs.google.com/spreadsheets/d/1oWS7cao-fgz2MKWtyr8h2dEL9unX__0bJrWKv6mQmM4/edit#gid=1099484640)" .

<https://example.org/ccdh/CancerGradeObservationSet> a owl:Class,
        linkml:ClassDefinition ;
    rdfs:label "CancerGradeObservationSet" ;
    rdfs:subClassOf [ a owl:Restriction ;
            owl:allValuesFrom <https://example.org/ccdh/Entity> ;
            owl:onProperty linkml:observations ],
        [ a owl:Restriction ;
            owl:maxQualifiedCardinality 1 ;
            owl:onClass <http://UNKNOWN.org/enum_CRDC-H.CancerGradeObservationSet.method_type> ;
            owl:onProperty linkml:method_type ],
        <https://example.org/ccdh/Entity> ;
    skos:definition "A structured object to hold related data items about the grade of cancer (e.g. overall, primary gleason, secondary gleason, etc.)." ;
    skos:editorialNote "Derived from [CancerGradeObservationSet in sheet CancerGradeSet](https://docs.google.com/spreadsheets/d/1oWS7cao-fgz2MKWtyr8h2dEL9unX__0bJrWKv6mQmM4/edit#gid=1025765903)" .

<https://example.org/ccdh/CcdhCode> a owl:Class,
        linkml:TypeDefinition ;
    rdfs:label "ccdh_code" ;
    rdfs:subClassOf linkml:String ;
    skos:editorialNote "Derived from [ccdh_code in sheet Primitives](https://docs.google.com/spreadsheets/d/1oWS7cao-fgz2MKWtyr8h2dEL9unX__0bJrWKv6mQmM4/edit#gid=497370447)" .

<https://example.org/ccdh/CcdhCurie> a owl:Class,
        linkml:TypeDefinition ;
    rdfs:label "ccdh_curie" ;
    rdfs:subClassOf linkml:Uriorcurie ;
    skos:definition " A compact URI (CURIE), which is a bipartite identifier of the form prefix:reference, in which the prefix is a convenient abbreviation of a URI.  It is expressed in the format “prefix:reference”. When a mapping of prefix to base URI is provided (external to this data type), a CURIE may be mapped to a URI." ;
    skos:editorialNote "Derived from [ccdh_curie in sheet Primitives](https://docs.google.com/spreadsheets/d/1oWS7cao-fgz2MKWtyr8h2dEL9unX__0bJrWKv6mQmM4/edit#gid=497370447)" .

<https://example.org/ccdh/CodeableConcept> a owl:Class,
        linkml:ClassDefinition ;
    rdfs:label "CodeableConcept" ;
    rdfs:subClassOf [ a owl:Restriction ;
            owl:maxQualifiedCardinality 1 ;
            owl:onClass <https://example.org/ccdh/CcdhString> ;
            owl:onProperty linkml:text ],
        [ a owl:Restriction ;
            owl:allValuesFrom <https://example.org/ccdh/Coding> ;
            owl:onProperty linkml:coding ],
        <https://example.org/ccdh/Entity> ;
    skos:definition "A representation of a concept that may be defined by or mapped to one or more codes in code systems (terminologies, ontologies, dictionaries, code sets, etc) - but may also be defined by the provision of text." ;
    skos:editorialNote "Derived from [CodeableConcept in sheet CodeableConcept](https://docs.google.com/spreadsheets/d/1oWS7cao-fgz2MKWtyr8h2dEL9unX__0bJrWKv6mQmM4/edit#gid=1820375300)" .

<https://example.org/ccdh/Exposure> a owl:Class,
        linkml:ClassDefinition ;
    rdfs:label "Exposure" ;
    rdfs:subClassOf [ a owl:Restriction ;
            owl:allValuesFrom <https://example.org/ccdh/Identifier> ;
            owl:onProperty linkml:identifier ],
        [ a owl:Restriction ;
            owl:allValuesFrom <https://example.org/ccdh/Entity> ;
            owl:onProperty linkml:tobacco_use ],
        [ a owl:Restriction ;
            owl:allValuesFrom <https://example.org/ccdh/Observation> ;
            owl:onProperty linkml:environmental ],
        [ a owl:Restriction ;
            owl:onClass <https://example.org/ccdh/CcdhString> ;
            owl:onProperty linkml:id ;
            owl:qualifiedCardinality 1 ],
        [ a owl:Restriction ;
            owl:maxQualifiedCardinality 1 ;
            owl:onClass <https://example.org/ccdh/Entity> ;
            owl:onProperty linkml:alcohol_use ],
        [ a owl:Restriction ;
            owl:maxQualifiedCardinality 1 ;
            owl:onClass <https://example.org/ccdh/Subject> ;
            owl:onProperty linkml:subject ],
        <https://example.org/ccdh/Entity> ;
    skos:definition "Contact between an agent and a target. A state of contact or close proximity to a medicinal product, chemical, pathogen, radioisotope or other substance." ;
    skos:editorialNote "Derived from [Exposure in sheet Exposure](https://docs.google.com/spreadsheets/d/1oWS7cao-fgz2MKWtyr8h2dEL9unX__0bJrWKv6mQmM4/edit#gid=1402410931)" .

<https://example.org/ccdh/ResearchSubject> a owl:Class,
        linkml:ClassDefinition ;
    rdfs:label "ResearchSubject" ;
    rdfs:subClassOf [ a owl:Restriction ;
            owl:maxQualifiedCardinality 1 ;
            owl:onClass <http://UNKNOWN.org/enum_CRDC-H.ResearchSubject.index_timepoint> ;
            owl:onProperty linkml:index_timepoint ],
        [ a owl:Restriction ;
            owl:onClass <https://example.org/ccdh/Subject> ;
            owl:onProperty linkml:associated_subject ;
            owl:qualifiedCardinality 1 ],
        [ a owl:Restriction ;
            owl:maxQualifiedCardinality 1 ;
            owl:onClass <https://example.org/ccdh/Quantity> ;
            owl:onProperty linkml:age_at_enrollment ],
        [ a owl:Restriction ;
            owl:allValuesFrom <https://example.org/ccdh/Diagnosis> ;
            owl:onProperty linkml:comorbid_diagnoses ],
        [ a owl:Restriction ;
            owl:maxQualifiedCardinality 1 ;
            owl:onClass <http://UNKNOWN.org/enum_CRDC-H.ResearchSubject.primary_diagnosis_site> ;
            owl:onProperty linkml:primary_diagnosis_site ],
        [ a owl:Restriction ;
            owl:maxQualifiedCardinality 1 ;
            owl:onClass <https://example.org/ccdh/CcdhString> ;
            owl:onProperty linkml:description ],
        [ a owl:Restriction ;
            owl:allValuesFrom <https://example.org/ccdh/Diagnosis> ;
            owl:onProperty linkml:primary_diagnosis ],
        [ a owl:Restriction ;
            owl:onClass <https://example.org/ccdh/CcdhString> ;
            owl:onProperty linkml:id ;
            owl:qualifiedCardinality 1 ],
        [ a owl:Restriction ;
            owl:maxQualifiedCardinality 1 ;
            owl:onClass <https://example.org/ccdh/ResearchProject> ;
            owl:onProperty linkml:member_of_research_project ],
        [ a owl:Restriction ;
            owl:allValuesFrom <https://example.org/ccdh/Identifier> ;
            owl:onProperty linkml:identifier ],
        [ a owl:Restriction ;
            owl:maxQualifiedCardinality 1 ;
            owl:onClass <https://example.org/ccdh/Organization> ;
            owl:onProperty linkml:originating_site ],
        [ a owl:Restriction ;
            owl:maxQualifiedCardinality 1 ;
            owl:onClass <http://UNKNOWN.org/enum_CRDC-H.ResearchSubject.primary_diagnosis_condition> ;
            owl:onProperty linkml:primary_diagnosis_condition ],
        <https://example.org/ccdh/Entity> ;
    skos:definition """A research subject is the entity of interest in a research study, typically a human being or an animal, but can also be a device, group of humans or animals, 
or a tissue sample. Human research subjects are usually not traceable to a particular person to protect the subject’s privacy.""" ;
    skos:editorialNote "Derived from [ResearchSubject in sheet ResearchSubject](https://docs.google.com/spreadsheets/d/1oWS7cao-fgz2MKWtyr8h2dEL9unX__0bJrWKv6mQmM4/edit#gid=665511119)" .

<https://example.org/ccdh/TimePeriod> a owl:Class,
        linkml:ClassDefinition ;
    rdfs:label "TimePeriod" ;
    rdfs:subClassOf [ a owl:Restriction ;
            owl:maxQualifiedCardinality 1 ;
            owl:onClass <https://example.org/ccdh/TimePoint> ;
            owl:onProperty linkml:periodEnd_end ],
        [ a owl:Restriction ;
            owl:maxQualifiedCardinality 1 ;
            owl:onClass <https://example.org/ccdh/TimePoint> ;
            owl:onProperty linkml:periodStart_start ],
        <https://example.org/ccdh/Entity> ;
    skos:definition "" ;
    skos:editorialNote "Derived from [TimePeriod in sheet TimePeriod](https://docs.google.com/spreadsheets/d/1oWS7cao-fgz2MKWtyr8h2dEL9unX__0bJrWKv6mQmM4/edit#gid=1590126992)" .

linkml:Date a owl:Class,
        linkml:TypeDefinition ;
    rdfs:label "date" ;
    rdfs:subClassOf [ a owl:Restriction ;
            owl:onDataRange xsd:date ;
            owl:onProperty linkml:topValue ;
            owl:qualifiedCardinality 1 ] ;
    skos:definition "a date (year, month and day) in an idealized calendar" ;
    skos:editorialNote "URI is dateTime because OWL reasoners don't work with straight date or time" .

linkml:Double a owl:Class,
        linkml:TypeDefinition ;
    rdfs:label "double" ;
    rdfs:subClassOf [ a owl:Restriction ;
            owl:onDataRange xsd:double ;
            owl:onProperty linkml:topValue ;
            owl:qualifiedCardinality 1 ] ;
    skos:definition "A real number that conforms to the xsd:double specification" .

linkml:Float a owl:Class,
        linkml:TypeDefinition ;
    rdfs:label "float" ;
    rdfs:subClassOf [ a owl:Restriction ;
            owl:onDataRange xsd:float ;
            owl:onProperty linkml:topValue ;
            owl:qualifiedCardinality 1 ] ;
    skos:definition "A real number that conforms to the xsd:float specification" .

linkml:Ncname a owl:Class,
        linkml:TypeDefinition ;
    rdfs:label "ncname" ;
    rdfs:subClassOf [ a owl:Restriction ;
            owl:onDataRange xsd:string ;
            owl:onProperty linkml:topValue ;
            owl:qualifiedCardinality 1 ] ;
    skos:definition "Prefix part of CURIE" .

linkml:Nodeidentifier a owl:Class,
        linkml:TypeDefinition ;
    rdfs:label "nodeidentifier" ;
    rdfs:subClassOf [ a owl:Restriction ;
            owl:onDataRange <http://www.w3.org/ns/shex#nonLiteral> ;
            owl:onProperty linkml:topValue ;
            owl:qualifiedCardinality 1 ] ;
    skos:definition "A URI, CURIE or BNODE that represents a node in a model." .

linkml:Objectidentifier a owl:Class,
        linkml:TypeDefinition ;
    rdfs:label "objectidentifier" ;
    rdfs:subClassOf [ a owl:Restriction ;
            owl:onDataRange <http://www.w3.org/ns/shex#iri> ;
            owl:onProperty linkml:topValue ;
            owl:qualifiedCardinality 1 ] ;
    skos:definition "A URI or CURIE that represents an object in the model." ;
    skos:note "Used for inheritence and type checking" .

linkml:SubsetDefinition a owl:Class ;
    rdfs:label "subset_definition" ;
    skos:definition "the name and description of a subset" .

linkml:Time a owl:Class,
        linkml:TypeDefinition ;
    rdfs:label "time" ;
    rdfs:subClassOf [ a owl:Restriction ;
            owl:onDataRange xsd:dateTime ;
            owl:onProperty linkml:topValue ;
            owl:qualifiedCardinality 1 ] ;
    skos:definition "A time object represents a (local) time of day, independent of any particular day" ;
    skos:editorialNote "URI is dateTime because OWL reasoners don't work with straight date or time" .

linkml:Uri a owl:Class,
        linkml:TypeDefinition ;
    rdfs:label "uri" ;
    rdfs:subClassOf [ a owl:Restriction ;
            owl:onDataRange xsd:anyURI ;
            owl:onProperty linkml:topValue ;
            owl:qualifiedCardinality 1 ] ;
    skos:definition "a complete URI" .

linkml:biologicProduct__description a owl:ObjectProperty,
        linkml:SlotDefinition ;
    rdfs:label "biologicProduct__description" ;
    rdfs:range <https://example.org/ccdh/CcdhString> ;
    skos:definition "A free text field to capture additional info/explanation about the model system" ;
    skos:editorialNote "Cardinality: 0..1" .

linkml:biologicProduct__growth_rate a owl:ObjectProperty,
        linkml:SlotDefinition ;
    rdfs:label "biologicProduct__growth_rate" ;
    rdfs:range <https://example.org/ccdh/CcdhString> ;
    skos:definition "When the specimen an actively growing model system, such as a cell or tissue culture, this property captures its rate of growth." .

linkml:biologicProduct__id a owl:ObjectProperty,
        linkml:SlotDefinition ;
    rdfs:label "biologicProduct__id" ;
    rdfs:range <https://example.org/ccdh/CcdhString> ;
    skos:definition "The 'logical' identifier of the entity in the system of record.  This 'id' is guaranteed to be unique only within a given system, but not globally. The identified entity may have a different 'id' in a different system, and have many external business 'identifiers' associated with it." ;
    skos:editorialNote "Cardinality: 0..1" .

linkml:biologicProduct__identifier a owl:ObjectProperty,
        linkml:SlotDefinition ;
    rdfs:label "biologicProduct__identifier" ;
    rdfs:range <https://example.org/ccdh/Identifier> ;
    skos:definition "A 'business' identifier  or accession number for the entity, typically as provided by an external system or authority, that us globally unique and persists across implementing systems." ;
    skos:editorialNote "Cardinality: 0..m" .

linkml:biologicProduct__passage_number a owl:ObjectProperty,
        linkml:SlotDefinition ;
    rdfs:label "biologicProduct__passage_number" ;
    rdfs:range <https://example.org/ccdh/CcdhInteger> ;
    skos:definition "When the specimen an actively growing model system, such as a cell or tissue culture, this property captures its passage number." .

linkml:biologicProduct__product_type a owl:ObjectProperty,
        linkml:SlotDefinition ;
    rdfs:label "biologicProduct__product_type" ;
    rdfs:range <http://UNKNOWN.org/enum_CRDC-H.BiologicProduct.product_type> ;
    skos:definition "The high level type of model system (e.g. cell line, cell culture, tissue culture, organoid)" ;
    skos:editorialNote "Cardinality: 0..1" .

linkml:bodySite__qualifier a owl:ObjectProperty,
        linkml:SlotDefinition ;
    rdfs:label "bodySite__qualifier" ;
    rdfs:range <http://UNKNOWN.org/enum_CRDC-H.BodySite.qualifier> ;
    skos:definition "A qualifier that further refines or specifies the location of the body site (e.g. to indicate laterality, upper v. lower, containment, etc)." ;
    skos:editorialNote "Cardinality: 0..m" .

linkml:bodySite__site a owl:ObjectProperty,
        linkml:SlotDefinition ;
    rdfs:label "bodySite__site" ;
    rdfs:range <http://UNKNOWN.org/enum_CRDC-H.BodySite.site> ;
    skos:definition "A term describing any site in the body." ;
    skos:editorialNote "Cardinality: 1..1" .

linkml:cancerGradeObservationSet__method_type a owl:ObjectProperty,
        linkml:SlotDefinition ;
    rdfs:label "cancerGradeObservationSet__method_type" ;
    rdfs:range <http://UNKNOWN.org/enum_CRDC-H.CancerGradeObservationSet.method_type> ;
    skos:definition "The cancer grade classification system being used to classify the cancer (e.g. INPC, Gleason, etc.)" ;
    skos:editorialNote "Cardinality: 0..1" .

linkml:cancerGradeObservationSet__observations a owl:ObjectProperty,
        linkml:SlotDefinition ;
    rdfs:label "cancerGradeObservationSet__observations" ;
    rdfs:range <https://example.org/ccdh/Entity> ;
    skos:definition "The value from the grade classification system that classifies the cancer (e.g. Poorly differentiated, differntiated, etc.)" ;
    skos:editorialNote "Cardinality: 0..m" .

linkml:cancerGradeObservation__observation_type a owl:ObjectProperty,
        linkml:SlotDefinition ;
    rdfs:label "cancerGradeObservation__observation_type" ;
    rdfs:range <http://UNKNOWN.org/enum_CRDC-H.CancerGradeObservation.observation_type> ;
    skos:definition "The cancer grade classification system being used to classify the cancer (e.g. INPC, Gleason, etc.)" ;
    skos:editorialNote "Cardinality: 1..1" .

linkml:cancerGradeObservation__valueCodeableConcept a owl:ObjectProperty,
        linkml:SlotDefinition ;
    rdfs:label "cancerGradeObservation__valueCodeableConcept" ;
    rdfs:range <http://UNKNOWN.org/enum_CRDC-H.CancerGradeObservation.valueCodeableConcept> ;
    skos:definition "The value from the grade classification system that classifies the cancer (e.g. Poorly differentiated, differntiated, etc.)" ;
    skos:editorialNote "Cardinality: 0..1" .

linkml:cancerStageObservationSet__category a owl:ObjectProperty,
        linkml:SlotDefinition ;
    rdfs:label "cancerStageObservationSet__category" ;
    rdfs:range <http://UNKNOWN.org/enum_CRDC-H.CancerStageObservationSet.category> ;
    skos:definition "" ;
    skos:editorialNote "Cardinality: 1..1" .

linkml:cancerStageObservationSet__method_type a owl:ObjectProperty,
        linkml:SlotDefinition ;
    rdfs:label "cancerStageObservationSet__method_type" ;
    rdfs:range <http://UNKNOWN.org/enum_CRDC-H.CancerStageObservationSet.method_type> ;
    skos:definition "A type of method used in generating each of the Observations bundled in the set, in this case, the particular staging system being used to classify the cancer." ;
    skos:editorialNote "Cardinality: 0..1" .

linkml:cancerStageObservationSet__observations a owl:ObjectProperty,
        linkml:SlotDefinition ;
    rdfs:label "cancerStageObservationSet__observations" ;
    rdfs:range <https://example.org/ccdh/CancerStageObservation> ;
    skos:definition "A set of one or more more atomic observations about the cancer stage" ;
    skos:editorialNote "Cardinality: 0..m" .

linkml:cancerStageObservation__observation_type a owl:ObjectProperty,
        linkml:SlotDefinition ;
    rdfs:label "cancerStageObservation__observation_type" ;
    rdfs:range <http://UNKNOWN.org/enum_CRDC-H.CancerStageObservation.observation_type> ;
    skos:definition "The type of cancer staging component being represented (e.g. 'Clinical Metastasis (M)')" ;
    skos:editorialNote "Cardinality: 1..1" .

linkml:cancerStageObservation__valueCodeableConcept a owl:ObjectProperty,
        linkml:SlotDefinition ;
    rdfs:label "cancerStageObservation__valueCodeableConcept" ;
    rdfs:range <http://UNKNOWN.org/enum_CRDC-H.CancerStageObservation.valueCodeableConcept> ;
    skos:definition "The value for a cancer staging component being represented (e.g. 'M1')" ;
    skos:editorialNote "Cardinality: 0..1" .

linkml:codeableConcept__coding a owl:ObjectProperty,
        linkml:SlotDefinition ;
    rdfs:label "codeableConcept__coding" ;
    rdfs:range <https://example.org/ccdh/Coding> ;
    skos:definition "A reference to a code defined by a terminology system" ;
    skos:editorialNote "Cardinality: 0..m" .

linkml:codeableConcept__text a owl:ObjectProperty,
        linkml:SlotDefinition ;
    rdfs:label "codeableConcept__text" ;
    rdfs:range <https://example.org/ccdh/CcdhString> ;
    skos:definition "A human language representation of the concept represented by the Coding." ;
    skos:editorialNote "Cardinality: 0..1" .

linkml:coding__code a owl:ObjectProperty,
        linkml:SlotDefinition ;
    rdfs:label "coding__code" ;
    rdfs:range <https://example.org/ccdh/CcdhString> ;
    skos:definition "The symbol/value of the code, as defined by the code system." ;
    skos:editorialNote "Cardinality: 1..1" .

linkml:coding__label a owl:ObjectProperty,
        linkml:SlotDefinition ;
    rdfs:label "coding__label" ;
    rdfs:range <https://example.org/ccdh/CcdhString> ;
    skos:definition "A human-readable name for the code, as defined by the code system." ;
    skos:editorialNote "Cardinality: 0..1" .

linkml:coding__system a owl:ObjectProperty,
        linkml:SlotDefinition ;
    rdfs:label "coding__system" ;
    rdfs:range <https://example.org/ccdh/CcdhString> ;
    skos:definition "The code system where the code is defined." ;
    skos:editorialNote "Cardinality: 1..1" .

linkml:coding__systemURL a owl:ObjectProperty,
        linkml:SlotDefinition ;
    rdfs:label "coding__systemURL" ;
    rdfs:range <https://example.org/ccdh/CcdhString> ;
    skos:definition "A URL where the code system can be found." ;
    skos:editorialNote "Cardinality: 0..1" .

linkml:coding__systemVersion a owl:ObjectProperty,
        linkml:SlotDefinition ;
    rdfs:label "coding__systemVersion" ;
    rdfs:range <https://example.org/ccdh/CcdhString> ;
    skos:definition "The version of the code system." ;
    skos:editorialNote "Cardinality: 0..1" .

linkml:diagnosis__age_at_diagnosis a owl:ObjectProperty,
        linkml:SlotDefinition ;
    rdfs:label "diagnosis__age_at_diagnosis" ;
    rdfs:range <https://example.org/ccdh/Quantity> ;
    skos:definition "The age in days of the individual at the time of diagnosis" ;
    skos:editorialNote "Cardinality: 0..1" .

linkml:diagnosis__condition a owl:ObjectProperty,
        linkml:SlotDefinition ;
    rdfs:label "diagnosis__condition" ;
    rdfs:range <http://UNKNOWN.org/enum_CRDC-H.Diagnosis.condition> ;
    skos:definition "Code that captures the condition being diagnosed (e.g. ICD-O, ICD-10, SNOMED, etc.)" ;
    skos:editorialNote "Cardinality: 0..1" .

linkml:diagnosis__disease_status a owl:ObjectProperty,
        linkml:SlotDefinition ;
    rdfs:label "diagnosis__disease_status" ;
    rdfs:range <http://UNKNOWN.org/enum_CRDC-H.Diagnosis.disease_status> ;
    skos:definition "A term that refers to the nature and/or clinical outcome of a disease (e.g., primary disease, metastatic disease, recurrent disease, etc.)" ;
    skos:editorialNote "Cardinality: 0..1" .

linkml:diagnosis__grade a owl:ObjectProperty,
        linkml:SlotDefinition ;
    rdfs:label "diagnosis__grade" ;
    rdfs:range <https://example.org/ccdh/Entity> ;
    skos:definition "The degree of abnormality of cancer cells, a measure of differentiation, the extent to which cancer cells are similar in appearance and function to healthy cells of the same tissue type. The degree of differentiation often relates to the clinical behavior of the particular tumor. Based on the microscopic findings, tumor grade is commonly described by one of four degrees of severity. Histopathologic grade of a tumor may be used to plan treatment and estimate the future course, outcome, and overall prognosis of disease. Certain types of cancers, such as soft tissue sarcoma, primary brain tumors, lymphomas, and breast have special grading systems." ;
    skos:editorialNote "Cardinality: 0..m" .

linkml:diagnosis__id a owl:ObjectProperty,
        linkml:SlotDefinition ;
    rdfs:label "diagnosis__id" ;
    rdfs:range <https://example.org/ccdh/CcdhString> ;
    skos:definition "The 'logical' identifier of the entity in the system of record, e.g. a UUID.  This 'id' is unique within a given system of record. The identified entity may have a different 'id' in a different system." ;
    skos:editorialNote "Cardinality: 0..1" .

linkml:diagnosis__identifier a owl:ObjectProperty,
        linkml:SlotDefinition ;
    rdfs:label "diagnosis__identifier" ;
    rdfs:range <https://example.org/ccdh/Identifier> ;
    skos:definition "A 'business' identifier  or accession number for the entity, typically as provided by an external system or authority, that persists across implementing systems." ;
    skos:editorialNote "Cardinality: 0..m" .

linkml:diagnosis__metastatic_site a owl:ObjectProperty,
        linkml:SlotDefinition ;
    rdfs:label "diagnosis__metastatic_site" ;
    rdfs:range <https://example.org/ccdh/BodySite> ;
    skos:definition "The anatomical location(s) of metastatic disease" ;
    skos:editorialNote "Cardinality: 0..m" .

linkml:diagnosis__method_of_diagnosis a owl:ObjectProperty,
        linkml:SlotDefinition ;
    rdfs:label "diagnosis__method_of_diagnosis" ;
    rdfs:range <http://UNKNOWN.org/enum_CRDC-H.Diagnosis.method_of_diagnosis> ;
    skos:definition "The method used to confirm the patients malignant diagnosis" ;
    skos:editorialNote "Cardinality: 0..1" .

linkml:diagnosis__morphology a owl:ObjectProperty,
        linkml:SlotDefinition ;
    rdfs:label "diagnosis__morphology" ;
    rdfs:range <http://UNKNOWN.org/enum_CRDC-H.Diagnosis.morphology> ;
    skos:definition "Code that represents the histology of the disease using the third edition of the International Classification of Diseases for Oncology, published in 2000, used principally in tumor and cancer registries for coding the site (topography) and the histology (morphology) of neoplasms." ;
    skos:editorialNote "Cardinality: 0..1" .

linkml:diagnosis__primary_site a owl:ObjectProperty,
        linkml:SlotDefinition ;
    rdfs:label "diagnosis__primary_site" ;
    rdfs:range <https://example.org/ccdh/BodySite> ;
    skos:definition "The anatomical location of the primary condition" ;
    skos:editorialNote "Cardinality: 0..m" .

linkml:diagnosis__prior_diagnosis a owl:ObjectProperty,
        linkml:SlotDefinition ;
    rdfs:label "diagnosis__prior_diagnosis" ;
    rdfs:range <https://example.org/ccdh/Diagnosis> ;
    skos:definition "A reference to a prior cancer diagnosis.  In the case of relapse/recurrent disease, this attribute may be populated with a reference to the intial diagnosis." ;
    skos:editorialNote "Cardinality: 0..1" .

linkml:diagnosis__related_specimen a owl:ObjectProperty,
        linkml:SlotDefinition ;
    rdfs:label "diagnosis__related_specimen" ;
    rdfs:range <https://example.org/ccdh/Specimen> ;
    skos:definition "The specimen from which this diagnosis is made" ;
    skos:editorialNote "Cardinality: 0..m" .

linkml:diagnosis__stage a owl:ObjectProperty,
        linkml:SlotDefinition ;
    rdfs:label "diagnosis__stage" ;
    rdfs:range <https://example.org/ccdh/CancerStageObservationSet> ;
    skos:definition "The extent of a cancer in the body. Staging is usually based on the size of the tumor, whether lymph nodes contain cancer, and whether the cancer has spread from the original site to other parts of the body." ;
    skos:editorialNote "Cardinality: 0..m" .

linkml:diagnosis__year_at_diagnosis a owl:ObjectProperty,
        linkml:SlotDefinition ;
    rdfs:label "diagnosis__year_at_diagnosis" ;
    rdfs:range <https://example.org/ccdh/CcdhInteger> ;
    skos:definition "Numeric value to represent the year of an individual's diagnosis." ;
    skos:editorialNote "Cardinality: 0..1" .

linkml:document__description a owl:ObjectProperty,
        linkml:SlotDefinition ;
    rdfs:label "document__description" ;
    rdfs:range <https://example.org/ccdh/CcdhString> ;
    skos:definition "A free text description or summary of the report." ;
    skos:editorialNote "Cardinality: 0..1" .

linkml:document__document_type a owl:ObjectProperty,
        linkml:SlotDefinition ;
    rdfs:label "document__document_type" ;
    rdfs:range <http://UNKNOWN.org/enum_CRDC-H.Document.document_type> ;
    skos:definition "The high-level type of the report (e.g. 'pathology report')" ;
    skos:editorialNote "Cardinality: 0..1" .

linkml:document__focus a owl:ObjectProperty,
        linkml:SlotDefinition ;
    rdfs:label "document__focus" ;
    rdfs:range <https://example.org/ccdh/Entity> ;
    skos:definition "The entity that the report is primarily about" ;
    skos:editorialNote "Cardinality: 0..1" .

linkml:document__id a owl:ObjectProperty,
        linkml:SlotDefinition ;
    rdfs:label "document__id" ;
    rdfs:range <https://example.org/ccdh/CcdhString> ;
    skos:definition "The 'logical' identifier of the entity in the system of record.  This 'id' is guaranteed to be unique only within a given system, but not globally. The identified entity may have a different 'id' in a different system, and have many external business 'identifiers' associated with it." ;
    skos:editorialNote "Cardinality: 0..1" .

linkml:document__identifier a owl:ObjectProperty,
        linkml:SlotDefinition ;
    rdfs:label "document__identifier" ;
    rdfs:range <https://example.org/ccdh/Identifier> ;
    skos:definition "A 'business' identifier  or accession number for the entity, typically as provided by an external system or authority, that us globally unique and persists across implementing systems." ;
    skos:editorialNote "Cardinality: 0..m" .

linkml:document__url a owl:ObjectProperty,
        linkml:SlotDefinition ;
    rdfs:label "document__url" ;
    rdfs:range <https://example.org/ccdh/CcdhString> ;
    skos:definition "A URL/web address where the document can be accessed." ;
    skos:editorialNote "Cardinality: 0..m" .

linkml:entity__id a owl:ObjectProperty,
        linkml:SlotDefinition ;
    rdfs:label "entity__id" ;
    rdfs:range <https://example.org/ccdh/CcdhString> ;
    skos:definition "The 'logical' identifier of the entity in the system of record, e.g. a UUID.  This 'id' is unique within a given system of record. The identified entity (with same \"identifier\" value for example) may have a different 'id' in a different system." ;
    skos:editorialNote "Cardinality: 0..1" .

linkml:exposure__alcohol_use a owl:ObjectProperty,
        linkml:SlotDefinition ;
    rdfs:label "exposure__alcohol_use" ;
    rdfs:range <https://example.org/ccdh/Entity> ;
    skos:definition "A container holding a set of observations about an individual's exposure to alcohol." ;
    skos:editorialNote "Cardinality: 0..1" .

linkml:exposure__environmental a owl:ObjectProperty,
        linkml:SlotDefinition ;
    rdfs:label "exposure__environmental" ;
    rdfs:range <https://example.org/ccdh/Observation> ;
    skos:definition "Observations about an individual's exposure to environmental substances that may impact clinical outcomes." ;
    skos:editorialNote "Cardinality: 0..m" .

linkml:exposure__id a owl:ObjectProperty,
        linkml:SlotDefinition ;
    rdfs:label "exposure__id" ;
    rdfs:range <https://example.org/ccdh/CcdhString> ;
    skos:definition "The 'logical' identifier of the entity in the system of record.  This 'id' is guaranteed to be unique only within a given system, but not globally. The identified entity may have a different 'id' in a different system, and have many external business 'identifiers' associated with it." ;
    skos:editorialNote "Cardinality: 1..1" .

linkml:exposure__identifier a owl:ObjectProperty,
        linkml:SlotDefinition ;
    rdfs:label "exposure__identifier" ;
    rdfs:range <https://example.org/ccdh/Identifier> ;
    skos:definition "A 'business' identifier for the entity, typically as provided by an external system or authority, that persists across implementing systems." ;
    skos:editorialNote "Cardinality: 0..m" .

linkml:exposure__subject a owl:ObjectProperty,
        linkml:SlotDefinition ;
    rdfs:label "exposure__subject" ;
    rdfs:range <https://example.org/ccdh/Subject> ;
    skos:definition "A reference to the Subject that is the subject of this Exposure" ;
    skos:editorialNote "Cardinality: 0..1" .

linkml:exposure__tobacco_use a owl:ObjectProperty,
        linkml:SlotDefinition ;
    rdfs:label "exposure__tobacco_use" ;
    rdfs:range <https://example.org/ccdh/Entity> ;
    skos:definition "A container holding a set of observations about an individual's exposure to tobacco." ;
    skos:editorialNote "Cardinality: 0..m" .

linkml:identifier__system a owl:ObjectProperty,
        linkml:SlotDefinition ;
    rdfs:label "identifier__system" ;
    rdfs:range <https://example.org/ccdh/CcdhString> ;
    skos:definition "The system or namespace that defines the identifier." ;
    skos:editorialNote "Cardinality: 0..1" .

linkml:identifier__type a owl:ObjectProperty,
        linkml:SlotDefinition ;
    rdfs:label "identifier__type" ;
    rdfs:range <http://UNKNOWN.org/enum_CRDC-H.Identifier.type> ;
    skos:definition "A code that defines the type of the identifier." ;
    skos:editorialNote "Cardinality: 0..1" .

linkml:identifier__value a owl:ObjectProperty,
        linkml:SlotDefinition ;
    rdfs:label "identifier__value" ;
    rdfs:range <https://example.org/ccdh/CcdhString> ;
    skos:definition "The value of the identifier, as defined by the system." ;
    skos:editorialNote "Cardinality: 1..1" .

linkml:observation__category a owl:ObjectProperty,
        linkml:SlotDefinition ;
    rdfs:label "observation__category" ;
    rdfs:range <http://UNKNOWN.org/enum_CRDC-H.Observation.category> ;
    skos:definition "The general category of observation described" ;
    skos:editorialNote "Cardinality: 1..1" .

linkml:observation__focus a owl:ObjectProperty,
        linkml:SlotDefinition ;
    rdfs:label "observation__focus" ;
    rdfs:range <https://example.org/ccdh/Entity> ;
    skos:definition "The entity or entities directly observed/measured in generating an observation result." ;
    skos:editorialNote "Cardinality: 0..m" .

linkml:observation__id a owl:ObjectProperty,
        linkml:SlotDefinition ;
    rdfs:label "observation__id" ;
    rdfs:range <https://example.org/ccdh/CcdhString> ;
    skos:definition "The 'logical' identifier of the entity in the system of record.  This 'id' is guaranteed to be unique only within a given system, but not globally. The identified entity may have a different 'id' in a different system, and have many external business 'identifiers' associated with it." ;
    skos:editorialNote "Cardinality: 1..1" .

linkml:observation__method_type a owl:ObjectProperty,
        linkml:SlotDefinition ;
    rdfs:label "observation__method_type" ;
    rdfs:range <http://UNKNOWN.org/enum_CRDC-H.Observation.method_type> ;
    skos:definition "A type of method used in generating the Observation result." ;
    skos:editorialNote "Cardinality: 0..m" .

linkml:observation__observation_type a owl:ObjectProperty,
        linkml:SlotDefinition ;
    rdfs:label "observation__observation_type" ;
    rdfs:range <http://UNKNOWN.org/enum_CRDC-H.Observation.observation_type> ;
    skos:definition "The specific type of observation made - i.e. the feature or characteristic that was observed, measured, estimated, etc.." ;
    skos:editorialNote "Cardinality: 1..1" .

linkml:observation__performed_by a owl:ObjectProperty,
        linkml:SlotDefinition ;
    rdfs:label "observation__performed_by" ;
    rdfs:range <https://example.org/ccdh/Organization> ;
    skos:definition "The organization or group that performed the observation activity." ;
    skos:editorialNote "Cardinality: 0..1" .

linkml:observation__subject a owl:ObjectProperty,
        linkml:SlotDefinition ;
    rdfs:label "observation__subject" ;
    rdfs:range <https://example.org/ccdh/Subject> ;
    skos:definition "The patient that the observation is about (if not the direct focus).  e.g. observations are often made on specimens derived from a patient, or other entities related to a patient, that ultimately tell us something about the patient of interest." ;
    skos:editorialNote "Cardinality: 0..1" .

linkml:observation__valueBoolean a owl:ObjectProperty,
        linkml:SlotDefinition ;
    rdfs:label "observation__valueBoolean" ;
    rdfs:range <https://example.org/ccdh/CcdhBoolean> ;
    skos:definition "The result of the observation, encoded as a boolean." ;
    skos:editorialNote "Cardinality: 0..1" .

linkml:observation__valueCodeableConcept a owl:ObjectProperty,
        linkml:SlotDefinition ;
    rdfs:label "observation__valueCodeableConcept" ;
    rdfs:range <http://UNKNOWN.org/enum_CRDC-H.Observation.valueCodeableConcept> ;
    skos:definition "The result of the observation, encoded as a CodeableConcept." ;
    skos:editorialNote "Cardinality: 0..1" .

linkml:observation__valueDateTime a owl:ObjectProperty,
        linkml:SlotDefinition ;
    rdfs:label "observation__valueDateTime" ;
    rdfs:range <https://example.org/ccdh/CcdhDateTime> ;
    skos:definition "The result of the observation, encoded as a dateTime." ;
    skos:editorialNote "Cardinality: 0..1" .

linkml:observation__valueDecimal a owl:ObjectProperty,
        linkml:SlotDefinition ;
    rdfs:label "observation__valueDecimal" ;
    rdfs:range <https://example.org/ccdh/CcdhDecimal> ;
    skos:definition "The result of the observation, encoded as a decimal." ;
    skos:editorialNote "Cardinality: 0..1" .

linkml:observation__valueEntity a owl:ObjectProperty,
        linkml:SlotDefinition ;
    rdfs:label "observation__valueEntity" ;
    rdfs:range <https://example.org/ccdh/Entity> ;
    skos:definition "The value of an observation" ;
    skos:editorialNote "Cardinality: 0..1" .

linkml:observation__valueInteger a owl:ObjectProperty,
        linkml:SlotDefinition ;
    rdfs:label "observation__valueInteger" ;
    rdfs:range <https://example.org/ccdh/CcdhDecimal> ;
    skos:definition "The result of the observation, encoded as a decimal." ;
    skos:editorialNote "Cardinality: 0..1" .

linkml:observation__valueQuantity a owl:ObjectProperty,
        linkml:SlotDefinition ;
    rdfs:label "observation__valueQuantity" ;
    rdfs:range <https://example.org/ccdh/Quantity> ;
    skos:definition "The result of the observation, encoded as a free-text Quantity." ;
    skos:editorialNote "Cardinality: 0..1" .

linkml:observation__valueString a owl:ObjectProperty,
        linkml:SlotDefinition ;
    rdfs:label "observation__valueString" ;
    rdfs:range <https://example.org/ccdh/CcdhString> ;
    skos:definition "The result of the observation, encoded as a free-text string." ;
    skos:editorialNote "Cardinality: 0..1" .

linkml:organization__alias a owl:ObjectProperty,
        linkml:SlotDefinition ;
    rdfs:label "organization__alias" ;
    rdfs:range <https://example.org/ccdh/CcdhString> ;
    skos:definition "A secondary name for the organization such as a short name or abbreviation (e.g. 'NCI')" ;
    skos:editorialNote "Cardinality: 0..1" .

linkml:organization__id a owl:ObjectProperty,
        linkml:SlotDefinition ;
    rdfs:label "organization__id" ;
    rdfs:range <https://example.org/ccdh/CcdhString> ;
    skos:definition "The 'logical' identifier of the entity in the system of record.  This 'id' is guaranteed to be unique only within a given system, but not globally. The identified entity may have a different 'id' in a different system, and have many external business 'identifiers' associated with it." ;
    skos:editorialNote "Cardinality: 1..1" .

linkml:organization__identifier a owl:ObjectProperty,
        linkml:SlotDefinition ;
    rdfs:label "organization__identifier" ;
    rdfs:range <https://example.org/ccdh/Identifier> ;
    skos:definition "A 'business' identifier for the entity, typically as provided by an external system or authority, that persists across implementing systems." ;
    skos:editorialNote "Cardinality: 0..m" .

linkml:organization__name a owl:ObjectProperty,
        linkml:SlotDefinition ;
    rdfs:label "organization__name" ;
    rdfs:range <https://example.org/ccdh/CcdhString> ;
    skos:definition "The full legal name by which the organization is known (e.g. 'National Cancer Institute')" ;
    skos:editorialNote "Cardinality: 0..1" .

linkml:organization__organization_type a owl:ObjectProperty,
        linkml:SlotDefinition ;
    rdfs:label "organization__organization_type" ;
    rdfs:range <https://example.org/ccdh/CcdhString> ;
    skos:definition "The type of the organization (e.g. 'Cancer Genome Characterization Center')" ;
    skos:editorialNote "Cardinality: 0..1" .

linkml:quantity__comparator a owl:ObjectProperty,
        linkml:SlotDefinition ;
    rdfs:label "quantity__comparator" ;
    rdfs:range <https://example.org/ccdh/Coding> ;
    skos:definition "How to understand the value (e.g.  <  |  <=  |  =  |   >=  |  > )" ;
    skos:editorialNote "Cardinality: 0..1" .

linkml:quantity__unit a owl:ObjectProperty,
        linkml:SlotDefinition ;
    rdfs:label "quantity__unit" ;
    rdfs:range <https://example.org/ccdh/CcdhString> ;
    skos:definition "The unit of the amount represented by the value (e.g. mg, mL, days).  This may be a free-text form of the unitCode." ;
    skos:editorialNote "Cardinality: 0..1" .

linkml:quantity__unitCode a owl:ObjectProperty,
        linkml:SlotDefinition ;
    rdfs:label "quantity__unitCode" ;
    rdfs:range <https://example.org/ccdh/Coding> ;
    skos:definition "A coded representation of the unit." ;
    skos:editorialNote "Cardinality: 0..1" .

linkml:quantity__valueCodeableConcept a owl:ObjectProperty,
        linkml:SlotDefinition ;
    rdfs:label "quantity__valueCodeableConcept" ;
    rdfs:range <http://UNKNOWN.org/enum_CRDC-H.Quantity.valueCodeableConcept> ;
    skos:definition "A coded value representing a quantity (e.g. \"Adjacent (< or = 2cm)\")" ;
    skos:editorialNote "Cardinality: 0..1" .

linkml:quantity__valueDecimal a owl:ObjectProperty,
        linkml:SlotDefinition ;
    rdfs:label "quantity__valueDecimal" ;
    rdfs:range <https://example.org/ccdh/CcdhDecimal> ;
    skos:definition "An amount, in the given units (if specified)" ;
    skos:editorialNote "Cardinality: 0..1" .

linkml:researchProject__date_ended a owl:ObjectProperty,
        linkml:SlotDefinition ;
    rdfs:label "researchProject__date_ended" ;
    rdfs:range <https://example.org/ccdh/CcdhDateTime> ;
    skos:definition "The date when the research project ended." ;
    skos:editorialNote "Cardinality: 0..1" .

linkml:researchProject__date_iacuc_approval a owl:ObjectProperty,
        linkml:SlotDefinition ;
    rdfs:label "researchProject__date_iacuc_approval" ;
    rdfs:range <https://example.org/ccdh/CcdhDateTime> ;
    skos:definition "The date that the Institutional Animal Care and Use Committee (IACUC) approved an animal study protocol. This date cannot be released to funding agencies until congruency between the animal use in the funding proposal and the IACUC approved protocol has been verified." ;
    skos:editorialNote "Cardinality: 0..1" .

linkml:researchProject__date_started a owl:ObjectProperty,
        linkml:SlotDefinition ;
    rdfs:label "researchProject__date_started" ;
    rdfs:range <https://example.org/ccdh/CcdhDateTime> ;
    skos:definition "The date when the research project began." ;
    skos:editorialNote "Cardinality: 0..1" .

linkml:researchProject__description a owl:ObjectProperty,
        linkml:SlotDefinition ;
    rdfs:label "researchProject__description" ;
    rdfs:range <https://example.org/ccdh/CcdhString> ;
    skos:definition "An unabridged description of a research program, project, or study." ;
    skos:editorialNote "Cardinality: 0..1" .

linkml:researchProject__description_shortened a owl:ObjectProperty,
        linkml:SlotDefinition ;
    rdfs:label "researchProject__description_shortened" ;
    rdfs:range <https://example.org/ccdh/CcdhString> ;
    skos:definition "An abbreviated description of a research program, project, or study." ;
    skos:editorialNote "Cardinality: 0..1" .

linkml:researchProject__id a owl:ObjectProperty,
        linkml:SlotDefinition ;
    rdfs:label "researchProject__id" ;
    rdfs:range <https://example.org/ccdh/CcdhString> ;
    skos:definition "The 'logical' identifier of the entity in the system of record.  This 'id' is guaranteed to be unique only within a given system, but not globally. The identified entity may have a different 'id' in a different system, and have many external business 'identifiers' associated with it." ;
    skos:editorialNote "Cardinality: 0..1" .

linkml:researchProject__identifier a owl:ObjectProperty,
        linkml:SlotDefinition ;
    rdfs:label "researchProject__identifier" ;
    rdfs:range <https://example.org/ccdh/Identifier> ;
    skos:definition "A 'business' identifier  or accession number for the entity, typically as provided by an external system or authority, that persists across implementing systems." ;
    skos:editorialNote "Cardinality: 0..m" .

linkml:researchProject__name a owl:ObjectProperty,
        linkml:SlotDefinition ;
    rdfs:label "researchProject__name" ;
    rdfs:range <https://example.org/ccdh/CcdhString> ;
    skos:definition "An unabridged name of a research program, project, or study." ;
    skos:editorialNote "Cardinality: 0..1" .

linkml:researchProject__name_shortened a owl:ObjectProperty,
        linkml:SlotDefinition ;
    rdfs:label "researchProject__name_shortened" ;
    rdfs:range <https://example.org/ccdh/CcdhString> ;
    skos:definition "An abbreviated name of a research program, project, or study." ;
    skos:editorialNote "Cardinality: 0..1" .

linkml:researchProject__part_of a owl:ObjectProperty,
        linkml:SlotDefinition ;
    rdfs:label "researchProject__part_of" ;
    rdfs:range <https://example.org/ccdh/ResearchProject> ;
    skos:definition "A reference to a parent ResearchProject (e.g. a link to the overarching CPTAC ResearchProject from a substudy of CPTAC)" ;
    skos:editorialNote "Cardinality: 0..m" .

linkml:researchProject__primary_anatomic_site a owl:ObjectProperty,
        linkml:SlotDefinition ;
    rdfs:label "researchProject__primary_anatomic_site" ;
    rdfs:range <http://UNKNOWN.org/enum_CRDC-H.ResearchProject.primary_anatomic_site> ;
    skos:definition "The text term used to describe the general location of the malignant disease, as categorized by the World Health Organization's (WHO) International Classification of Diseases for Oncology (ICD-O).  In the context of ResearchProject, this attribute captures the anatomic sites of research interest." ;
    skos:editorialNote "Cardinality: 0..m" .

linkml:researchProject__research_project_type a owl:ObjectProperty,
        linkml:SlotDefinition ;
    rdfs:label "researchProject__research_project_type" ;
    rdfs:range <http://UNKNOWN.org/enum_CRDC-H.ResearchProject.research_project_type> ;
    skos:definition "The 'type' of ResearchProject represented (e.g. a broad-based Program like 'CPTAC' or a more focused Project like 'CPTAC PDAC Discovery Study')" ;
    skos:editorialNote "Cardinality: 1..1" .

linkml:researchProject__sponsor a owl:ObjectProperty,
        linkml:SlotDefinition ;
    rdfs:label "researchProject__sponsor" ;
    rdfs:range <https://example.org/ccdh/CcdhString> ;
    skos:definition "An entity that is responsible for the initiation, management, and/or financing of a research project." ;
    skos:editorialNote "Cardinality: 0..m" .

linkml:researchProject__url a owl:ObjectProperty,
        linkml:SlotDefinition ;
    rdfs:label "researchProject__url" ;
    rdfs:range <https://example.org/ccdh/CcdhString> ;
    skos:definition "A URL address for a resource that provides information about a research program, project, or study." ;
    skos:editorialNote "Cardinality: 0..m" .

linkml:researchSubject__age_at_enrollment a owl:ObjectProperty,
        linkml:SlotDefinition ;
    rdfs:label "researchSubject__age_at_enrollment" ;
    rdfs:range <https://example.org/ccdh/Quantity> ;
    skos:definition "The age in days when the Subject enrolled on the ResearchProject" ;
    skos:editorialNote "Cardinality: 0..1" .

linkml:researchSubject__associated_subject a owl:ObjectProperty,
        linkml:SlotDefinition ;
    rdfs:label "researchSubject__associated_subject" ;
    rdfs:range <https://example.org/ccdh/Subject> ;
    skos:definition "A reference to the Subject that is this ResearchSubject" ;
    skos:editorialNote "Cardinality: 1..1" .

linkml:researchSubject__comorbid_diagnoses a owl:ObjectProperty,
        linkml:SlotDefinition ;
    rdfs:label "researchSubject__comorbid_diagnoses" ;
    rdfs:range <https://example.org/ccdh/Diagnosis> ;
    skos:definition "One or more diagnosis instance that are comorbid with the primary_diagnosis that qualified a subject for inclusion on a ResearchProject" ;
    skos:editorialNote "Cardinality: 0..m" .

linkml:researchSubject__description a owl:ObjectProperty,
        linkml:SlotDefinition ;
    rdfs:label "researchSubject__description" ;
    rdfs:range <https://example.org/ccdh/CcdhString> ;
    skos:definition "A free text field to capture additional info/explanation about the research subject." ;
    skos:editorialNote "Cardinality: 0..1" .

linkml:researchSubject__id a owl:ObjectProperty,
        linkml:SlotDefinition ;
    rdfs:label "researchSubject__id" ;
    rdfs:range <https://example.org/ccdh/CcdhString> ;
    skos:definition "The 'logical' identifier of the entity in the system of record.  This 'id' is guaranteed to be unique only within a given system, but not globally. The identified entity may have a different 'id' in a different system, and have many external business 'identifiers' associated with it." ;
    skos:editorialNote "Cardinality: 1..1" .

linkml:researchSubject__identifier a owl:ObjectProperty,
        linkml:SlotDefinition ;
    rdfs:label "researchSubject__identifier" ;
    rdfs:range <https://example.org/ccdh/Identifier> ;
    skos:definition "A 'business' identifier for the entity, typically as provided by an external system or authority, that persists across implementing systems." ;
    skos:editorialNote "Cardinality: 0..m" .

linkml:researchSubject__index_timepoint a owl:ObjectProperty,
        linkml:SlotDefinition ;
    rdfs:label "researchSubject__index_timepoint" ;
    rdfs:range <http://UNKNOWN.org/enum_CRDC-H.ResearchSubject.index_timepoint> ;
    skos:definition "The text term used to describe the reference or anchor date used for date obfuscation, where a single date is obscured by creating one or more date ranges in relation to this date." ;
    skos:editorialNote "Cardinality: 0..1" .

linkml:researchSubject__member_of_research_project a owl:ObjectProperty,
        linkml:SlotDefinition ;
    rdfs:label "researchSubject__member_of_research_project" ;
    rdfs:range <https://example.org/ccdh/ResearchProject> ;
    skos:definition "A reference to the Study(s) of which this ResearchSubject is a member" ;
    skos:editorialNote "Cardinality: 0..1" .

linkml:researchSubject__originating_site a owl:ObjectProperty,
        linkml:SlotDefinition ;
    rdfs:label "researchSubject__originating_site" ;
    rdfs:range <https://example.org/ccdh/Organization> ;
    skos:definition "The Organization at which a subject was enrolled on a ResearchProject." ;
    skos:editorialNote "Cardinality: 0..1" .

linkml:researchSubject__primary_diagnosis a owl:ObjectProperty,
        linkml:SlotDefinition ;
    rdfs:label "researchSubject__primary_diagnosis" ;
    rdfs:range <https://example.org/ccdh/Diagnosis> ;
    skos:definition "The diagnosis instance that qualified a subject for inclusion on a ResearchProject" ;
    skos:editorialNote "Cardinality: 0..m" .

linkml:researchSubject__primary_diagnosis_condition a owl:ObjectProperty,
        linkml:SlotDefinition ;
    rdfs:label "researchSubject__primary_diagnosis_condition" ;
    rdfs:range <http://UNKNOWN.org/enum_CRDC-H.ResearchSubject.primary_diagnosis_condition> ;
    skos:definition "The text term used to describe the type of malignant disease, as categorized by the World Health Organization's (WHO) International Classification of Diseases for Oncology (ICD-O).   This attribute represents the disease that qualified the subject for inclusion on the ResearchProject" ;
    skos:editorialNote "Cardinality: 0..1" .

linkml:researchSubject__primary_diagnosis_site a owl:ObjectProperty,
        linkml:SlotDefinition ;
    rdfs:label "researchSubject__primary_diagnosis_site" ;
    rdfs:range <http://UNKNOWN.org/enum_CRDC-H.ResearchSubject.primary_diagnosis_site> ;
    skos:definition "The text term used to describe the primary site of disease, as categorized by the World Health Organization's (WHO) International Classification of Diseases for Oncology (ICD-O). This categorization groups cases into general categories.  This attribute represents the primary site of disease that qualified the subject for inclusion on the ResearchProject." ;
    skos:editorialNote "Cardinality: 0..1" .

linkml:specimenContainer__additive a owl:ObjectProperty,
        linkml:SlotDefinition ;
    rdfs:label "specimenContainer__additive" ;
    rdfs:range <https://example.org/ccdh/Substance> ;
    skos:definition "A material substance added to the container (typically to support the primary object contained)" ;
    skos:editorialNote "Cardinality: 0..m" .

linkml:specimenContainer__charge_type a owl:ObjectProperty,
        linkml:SlotDefinition ;
    rdfs:label "specimenContainer__charge_type" ;
    rdfs:range <http://UNKNOWN.org/enum_CRDC-H.SpecimenContainer.charge_type> ;
    skos:definition "A descripton of the type of charge on a slide on which a specimen is mounted" ;
    skos:editorialNote "Cardinality: 0..1" .

linkml:specimenContainer__container_number a owl:ObjectProperty,
        linkml:SlotDefinition ;
    rdfs:label "specimenContainer__container_number" ;
    rdfs:range <https://example.org/ccdh/CcdhString> ;
    skos:definition "Informal number/identifier by which the container is referenced (e.g. a slide number, or a well number in a plate)" ;
    skos:editorialNote "Cardinality: 0..1" .

linkml:specimenContainer__container_type a owl:ObjectProperty,
        linkml:SlotDefinition ;
    rdfs:label "specimenContainer__container_type" ;
    rdfs:range <http://UNKNOWN.org/enum_CRDC-H.SpecimenContainer.container_type> ;
    skos:definition "The kind of container associated with the specimen." ;
    skos:editorialNote "Cardinality: 0..1" .

linkml:specimenContainer__id a owl:ObjectProperty,
        linkml:SlotDefinition ;
    rdfs:label "specimenContainer__id" ;
    rdfs:range <https://example.org/ccdh/CcdhString> ;
    skos:definition "The 'logical' identifier of the entity in the system of record.  This 'id' is guaranteed to be unique only within a given system, but not globally. The identified entity may have a different 'id' in a different system, and have many external business 'identifiers' associated with it." ;
    skos:editorialNote "Cardinality: 0..1" .

linkml:specimenContainer__identifier a owl:ObjectProperty,
        linkml:SlotDefinition ;
    rdfs:label "specimenContainer__identifier" ;
    rdfs:range <https://example.org/ccdh/Identifier> ;
    skos:definition "A 'business' identifier  or accession number for the entity, typically as provided by an external system or authority, that us globally unique and persists across implementing systems." ;
    skos:editorialNote "Cardinality: 0..m" .

linkml:specimenContainer__parent_container a owl:ObjectProperty,
        linkml:SlotDefinition ;
    rdfs:label "specimenContainer__parent_container" ;
    rdfs:range <https://example.org/ccdh/SpecimenContainer> ;
    skos:definition "A larger container of which this container is a part (e.g. a single well in a 96-well plate)" ;
    skos:editorialNote "Cardinality: 0..m (should be 0..1?)" .

linkml:specimenCreationActivity__activity_type a owl:ObjectProperty,
        linkml:SlotDefinition ;
    rdfs:label "specimenCreationActivity__activity_type" ;
    rdfs:range <http://UNKNOWN.org/enum_CRDC-H.SpecimenCreationActivity.activity_type> ;
    skos:definition "The high-level type of creation activity" ;
    skos:editorialNote "Cardinality: 0..1" .

linkml:specimenCreationActivity__additive a owl:ObjectProperty,
        linkml:SlotDefinition ;
    rdfs:label "specimenCreationActivity__additive" ;
    rdfs:range <https://example.org/ccdh/Substance> ;
    skos:definition "A type of material or reagent used as input when creating the specimen" ;
    skos:editorialNote "Cardinality: 0..m" .

linkml:specimenCreationActivity__collection_method_type a owl:ObjectProperty,
        linkml:SlotDefinition ;
    rdfs:label "specimenCreationActivity__collection_method_type" ;
    rdfs:range <http://UNKNOWN.org/enum_CRDC-H.SpecimenCreationActivity.collection_method_type> ;
    skos:definition "A type of method followed in collecting a sample from its original source." ;
    skos:editorialNote "Cardinality: 0..1" .

linkml:specimenCreationActivity__collection_site a owl:ObjectProperty,
        linkml:SlotDefinition ;
    rdfs:label "specimenCreationActivity__collection_site" ;
    rdfs:range <https://example.org/ccdh/BodySite> ;
    skos:definition "A data container holding information about the anatomic source of a specimen, including its location in the body, and the approach route used to access it." ;
    skos:editorialNote "Cardinality: 0..1" .

linkml:specimenCreationActivity__date_ended a owl:ObjectProperty,
        linkml:SlotDefinition ;
    rdfs:label "specimenCreationActivity__date_ended" ;
    rdfs:range <https://example.org/ccdh/TimePoint> ;
    skos:definition "The date when the activity ended (in this case, a specimen creation event)." ;
    skos:editorialNote "Cardinality: 0..1" .

linkml:specimenCreationActivity__date_started a owl:ObjectProperty,
        linkml:SlotDefinition ;
    rdfs:label "specimenCreationActivity__date_started" ;
    rdfs:range <https://example.org/ccdh/TimePoint> ;
    skos:definition "The date when the activity began (in this case, a specimen creation event)." ;
    skos:editorialNote "Cardinality: 0..1" .

linkml:specimenCreationActivity__derivation_method_type a owl:ObjectProperty,
        linkml:SlotDefinition ;
    rdfs:label "specimenCreationActivity__derivation_method_type" ;
    rdfs:range <http://UNKNOWN.org/enum_CRDC-H.SpecimenCreationActivity.derivation_method_type> ;
    skos:definition "A type of method followed in deriving new specimens from an existing one." ;
    skos:editorialNote "Cardinality: 0..1" .

linkml:specimenCreationActivity__execution_observation a owl:ObjectProperty,
        linkml:SlotDefinition ;
    rdfs:label "specimenCreationActivity__execution_observation" ;
    rdfs:range <https://example.org/ccdh/Observation> ;
    skos:definition "Information describing how an activity was executed - e.g. environmental conditions in which it was performed, how long certain parts took to complete, etc." ;
    skos:editorialNote "Cardinality: 0..m" .

linkml:specimenCreationActivity__input_specimen a owl:ObjectProperty,
        linkml:SlotDefinition ;
    rdfs:label "specimenCreationActivity__input_specimen" ;
    rdfs:range <https://example.org/ccdh/Specimen> ;
    skos:definition "One or more existing specimens input into the specimen creation activity, from which a new specimen is derived (e.g. through portioning, aliquoting, sectioning, etc)" ;
    skos:editorialNote "Cardinality: 0..m" .

linkml:specimenCreationActivity__performed_by a owl:ObjectProperty,
        linkml:SlotDefinition ;
    rdfs:label "specimenCreationActivity__performed_by" ;
    rdfs:range <https://example.org/ccdh/Organization> ;
    skos:definition "The organization or group that performed the activity." ;
    skos:editorialNote "Cardinality: 0..1" .

linkml:specimenCreationActivity__quantity_collected a owl:ObjectProperty,
        linkml:SlotDefinition ;
    rdfs:label "specimenCreationActivity__quantity_collected" ;
    rdfs:range <https://example.org/ccdh/Quantity> ;
    skos:definition "The quantity of material in the specimen as originally collected from its original source material (prior to downstream portioning or processing)" ;
    skos:editorialNote "Cardinality: 0..1" .

linkml:specimenCreationActivity__specimen_order a owl:ObjectProperty,
        linkml:SlotDefinition ;
    rdfs:label "specimenCreationActivity__specimen_order" ;
    rdfs:range <https://example.org/ccdh/CcdhString> ;
    skos:definition "A numeric value that represents the sequential order of this creation activity relative to that of creation of other specimens from the same source material or parent specimen." ;
    skos:editorialNote "Cardinality: 0..1" .

linkml:specimenProcessingActivity__activity_type a owl:ObjectProperty,
        linkml:SlotDefinition ;
    rdfs:label "specimenProcessingActivity__activity_type" ;
    rdfs:range <http://UNKNOWN.org/enum_CRDC-H.SpecimenProcessingActivity.activity_type> ;
    skos:definition "The high-level type of processing activity" ;
    skos:editorialNote "Cardinality: 0..1" .

linkml:specimenProcessingActivity__additive a owl:ObjectProperty,
        linkml:SlotDefinition ;
    rdfs:label "specimenProcessingActivity__additive" ;
    rdfs:range <https://example.org/ccdh/Substance> ;
    skos:definition "A type of material or reagent used as input when processing the specimen" ;
    skos:editorialNote "Cardinality: 0..m" .

linkml:specimenProcessingActivity__date_ended a owl:ObjectProperty,
        linkml:SlotDefinition ;
    rdfs:label "specimenProcessingActivity__date_ended" ;
    rdfs:range <https://example.org/ccdh/TimePoint> ;
    skos:definition "The date when the activity began (in this case, a specimen processing event)." ;
    skos:editorialNote "Cardinality: 0..1" .

linkml:specimenProcessingActivity__date_started a owl:ObjectProperty,
        linkml:SlotDefinition ;
    rdfs:label "specimenProcessingActivity__date_started" ;
    rdfs:range <https://example.org/ccdh/TimePoint> ;
    skos:definition "The date when the activity began (in this case, a specimen processing event)." ;
    skos:editorialNote "Cardinality: 0..1" .

linkml:specimenProcessingActivity__duration a owl:ObjectProperty,
        linkml:SlotDefinition ;
    rdfs:label "specimenProcessingActivity__duration" ;
    rdfs:range <https://example.org/ccdh/Entity> ;
    skos:definition "The length of time over which the activity was performed." .

linkml:specimenProcessingActivity__execution_observation a owl:ObjectProperty,
        linkml:SlotDefinition ;
    rdfs:label "specimenProcessingActivity__execution_observation" ;
    rdfs:range <https://example.org/ccdh/Entity> ;
    skos:definition "Information describing how an activity was executed - e.g. environmental conditions in which it was performed, how long certain parts took to complete, etc." ;
    skos:editorialNote "Cardinality: 0..m" .

linkml:specimenProcessingActivity__method_type a owl:ObjectProperty,
        linkml:SlotDefinition ;
    rdfs:label "specimenProcessingActivity__method_type" ;
    rdfs:range <http://UNKNOWN.org/enum_CRDC-H.SpecimenProcessingActivity.method_type> ;
    skos:definition "A specific type of method or procedure performed to process the specimen" ;
    skos:editorialNote "Cardinality: 0..1" .

linkml:specimenProcessingActivity__performed_by a owl:ObjectProperty,
        linkml:SlotDefinition ;
    rdfs:label "specimenProcessingActivity__performed_by" ;
    rdfs:range <https://example.org/ccdh/Organization> ;
    skos:definition "The organization or group that performed the activity." ;
    skos:editorialNote "Cardinality: 0..1" .

linkml:specimenStorageActivity__container a owl:ObjectProperty,
        linkml:SlotDefinition ;
    rdfs:label "specimenStorageActivity__container" ;
    rdfs:range <https://example.org/ccdh/SpecimenContainer> ;
    skos:definition "A container in which the specimen is held or affixed during its storage." ;
    skos:editorialNote "Cardinality: 0..m" .

linkml:specimenStorageActivity__date_ended a owl:ObjectProperty,
        linkml:SlotDefinition ;
    rdfs:label "specimenStorageActivity__date_ended" ;
    rdfs:range <https://example.org/ccdh/TimePoint> ;
    skos:definition "The date when the activity ended (in this case, a storage event)." ;
    skos:editorialNote "Cardinality: 0..1" .

linkml:specimenStorageActivity__date_started a owl:ObjectProperty,
        linkml:SlotDefinition ;
    rdfs:label "specimenStorageActivity__date_started" ;
    rdfs:range <https://example.org/ccdh/TimePoint> ;
    skos:definition "The date when the activity began (in this case, a storage event)." ;
    skos:editorialNote "Cardinality: 0..1" .

linkml:specimenStorageActivity__duration a owl:ObjectProperty,
        linkml:SlotDefinition ;
    rdfs:label "specimenStorageActivity__duration" ;
    rdfs:range <https://example.org/ccdh/Quantity> ;
    skos:definition "The length of time over which the activity was performed." ;
    skos:editorialNote "Cardinality: 0..1" .

linkml:specimenStorageActivity__method_type a owl:ObjectProperty,
        linkml:SlotDefinition ;
    rdfs:label "specimenStorageActivity__method_type" ;
    rdfs:range <http://UNKNOWN.org/enum_CRDC-H.SpecimenStorageActivity.method_type> ;
    skos:definition "A specific type of method or procedure performed to store the specimen" ;
    skos:editorialNote "Cardinality: 0..1" .

linkml:specimenStorageActivity__performed_by a owl:ObjectProperty,
        linkml:SlotDefinition ;
    rdfs:label "specimenStorageActivity__performed_by" ;
    rdfs:range <https://example.org/ccdh/Organization> ;
    skos:definition "The organization or group that performed the activity." ;
    skos:editorialNote "Cardinality: 0..1" .

linkml:specimenTransportActivity__date_ended a owl:ObjectProperty,
        linkml:SlotDefinition ;
    rdfs:label "specimenTransportActivity__date_ended" ;
    rdfs:range <https://example.org/ccdh/TimePoint> ;
    skos:definition "The date when the activity ended (in this case, a transport event)." ;
    skos:editorialNote "Cardinality: 0..1" .

linkml:specimenTransportActivity__date_started a owl:ObjectProperty,
        linkml:SlotDefinition ;
    rdfs:label "specimenTransportActivity__date_started" ;
    rdfs:range <https://example.org/ccdh/TimePoint> ;
    skos:definition "The date when the activity began (in this case, a transport event)." ;
    skos:editorialNote "Cardinality: 0..1" .

linkml:specimenTransportActivity__duration a owl:ObjectProperty,
        linkml:SlotDefinition ;
    rdfs:label "specimenTransportActivity__duration" ;
    rdfs:range <https://example.org/ccdh/CcdhString> ;
    skos:definition "The length of time over which the activity was performed." .

linkml:specimenTransportActivity__execution_conditions a owl:ObjectProperty,
        linkml:SlotDefinition ;
    rdfs:label "specimenTransportActivity__execution_conditions" ;
    rdfs:range <https://example.org/ccdh/CcdhString> ;
    skos:definition "An environmental condition under which the activity is executed (in this case, a transport activity)." ;
    skos:editorialNote "Cardinality: 0..m" .

linkml:specimenTransportActivity__execution_observation a owl:ObjectProperty,
        linkml:SlotDefinition ;
    rdfs:label "specimenTransportActivity__execution_observation" ;
    rdfs:range <https://example.org/ccdh/Entity> ;
    skos:definition "Information describing how an activity was executed - e.g. environmental conditions in which it was performed, how long certain parts took to complete, etc." ;
    skos:editorialNote "Cardinality: 0..m" .

linkml:specimenTransportActivity__performed_by a owl:ObjectProperty,
        linkml:SlotDefinition ;
    rdfs:label "specimenTransportActivity__performed_by" ;
    rdfs:range <https://example.org/ccdh/Organization> ;
    skos:definition "The organization or group that performed the activity." ;
    skos:editorialNote "Cardinality: 0..1" .

linkml:specimenTransportActivity__transport_destination a owl:ObjectProperty,
        linkml:SlotDefinition ;
    rdfs:label "specimenTransportActivity__transport_destination" ;
    rdfs:range <https://example.org/ccdh/Organization> ;
    skos:definition "An organization (facility, site, lab, etc) to which the specimen is delivered as a result of the activity." ;
    skos:editorialNote "Cardinality: 0..1" .

linkml:specimenTransportActivity__transport_origin a owl:ObjectProperty,
        linkml:SlotDefinition ;
    rdfs:label "specimenTransportActivity__transport_origin" ;
    rdfs:range <https://example.org/ccdh/Organization> ;
    skos:definition "An organization (facility, site, lab, etc) from which the specimen was transported as a result of the activity." ;
    skos:editorialNote "Cardinality: 0..1" .

linkml:specimen__analyte_type a owl:ObjectProperty,
        linkml:SlotDefinition ;
    rdfs:label "specimen__analyte_type" ;
    rdfs:range <http://UNKNOWN.org/enum_CRDC-H.Specimen.analyte_type> ;
    skos:definition "For speciemens of type 'analyte' (or an 'aliquot' derived from an analyte), this is the category of chemcial the analyte of interest represents (e.g. DNA, RNA)" ;
    skos:editorialNote "Cardinality: 0..1" .

linkml:specimen__associated_project a owl:ObjectProperty,
        linkml:SlotDefinition ;
    rdfs:label "specimen__associated_project" ;
    rdfs:range <https://example.org/ccdh/ResearchProject> ;
    skos:definition "The Project associated with the specimen." ;
    skos:editorialNote "Cardinality: 0..1" .

linkml:specimen__cellular_composition_type a owl:ObjectProperty,
        linkml:SlotDefinition ;
    rdfs:label "specimen__cellular_composition_type" ;
    rdfs:range <http://UNKNOWN.org/enum_CRDC-H.Specimen.cellular_composition_type> ;
    skos:definition "A term describing the type of material comprising a specimen at a celluar level." ;
    skos:editorialNote "Cardinality: 0..1" .

linkml:specimen__contained_in a owl:ObjectProperty,
        linkml:SlotDefinition ;
    rdfs:label "specimen__contained_in" ;
    rdfs:range <https://example.org/ccdh/SpecimenContainer> ;
    skos:definition "A physical container in which a specimen is held or attached -  as storage for future use,  a substrate for growth (e.g. a cell culture dish), or a vessel to enable analysis (e.g. a microscope slide or 96-well plate)" ;
    skos:editorialNote "Cardinality: 0..1" .

linkml:specimen__creation_activity a owl:ObjectProperty,
        linkml:SlotDefinition ;
    rdfs:label "specimen__creation_activity" ;
    rdfs:range <https://example.org/ccdh/SpecimenCreationActivity> ;
    skos:definition "An activity or procedure through which a specimen was created, through removing material from an biological subject, or deriving material from an existing specimen." ;
    skos:editorialNote "Cardinality: 0..1" .

linkml:specimen__data_provider a owl:ObjectProperty,
        linkml:SlotDefinition ;
    rdfs:label "specimen__data_provider" ;
    rdfs:range <https://example.org/ccdh/Organization> ;
    skos:definition "The organization/center that provided data associated with a specimen." ;
    skos:editorialNote "Cardinality: 0..1" .

linkml:specimen__degree_of_dysplasia a owl:ObjectProperty,
        linkml:SlotDefinition ;
    rdfs:label "specimen__degree_of_dysplasia" ;
    rdfs:range <http://UNKNOWN.org/enum_CRDC-H.Specimen.degree_of_dysplasia> ;
    skos:definition "A term describing the nature/extent of abnormal cells  that are not cancer, as observed upon microscopic assessment of a specimen. Records the degree of dysplasia for the cyst or lesion under consideration." ;
    skos:editorialNote "Cardinality: 0..1" .

linkml:specimen__derived_product a owl:ObjectProperty,
        linkml:SlotDefinition ;
    rdfs:label "specimen__derived_product" ;
    rdfs:range <https://example.org/ccdh/BiologicProduct> ;
    skos:definition "A 'living' biologically active product (e.g. a cell culture, tissue culture, or organoid) that was generated from the specimen" ;
    skos:editorialNote "Cardinality: 0..m" .

linkml:specimen__description a owl:ObjectProperty,
        linkml:SlotDefinition ;
    rdfs:label "specimen__description" ;
    rdfs:range <https://example.org/ccdh/CcdhString> ;
    skos:definition "A free text field to capture additional information or explanation about the specimen." ;
    skos:editorialNote "Cardinality: 0..1" .

linkml:specimen__dimensional_measure a owl:ObjectProperty,
        linkml:SlotDefinition ;
    rdfs:label "specimen__dimensional_measure" ;
    rdfs:range <https://example.org/ccdh/Entity> ;
    skos:definition "An observation about the dimensions of an object, including lengths, areas, and volumes." ;
    skos:editorialNote "Cardinality: 0..1" .

linkml:specimen__distance_from_paired_specimen a owl:ObjectProperty,
        linkml:SlotDefinition ;
    rdfs:label "specimen__distance_from_paired_specimen" ;
    rdfs:range <https://example.org/ccdh/Quantity> ;
    skos:definition "The observed distance of the specimen from a 'paired specimen' in the body at the time of collection. (e.g. the distance between the in vivo location of a tumor tissue specimen and its paired normal specimen)" ;
    skos:editorialNote "Cardinality: 0..1" .

linkml:specimen__dysplasia_fraction a owl:ObjectProperty,
        linkml:SlotDefinition ;
    rdfs:label "specimen__dysplasia_fraction" ;
    rdfs:range <https://example.org/ccdh/CcdhString> ;
    skos:definition "Resulting value to represent the number of pieces of dysplasia divided by the total number of pieces." ;
    skos:editorialNote "Cardinality: 0..1" .

linkml:specimen__general_tissue_morphology a owl:ObjectProperty,
        linkml:SlotDefinition ;
    rdfs:label "specimen__general_tissue_morphology" ;
    rdfs:range <http://UNKNOWN.org/enum_CRDC-H.Specimen.general_tissue_morphology> ;
    skos:definition "A term describing at a high-level the kind of tissue collected in a specimen, with respect to disease status or proximity to tumor tissue (e.g. is it normal, abnormal, tumor, tumor-adjacent)." ;
    skos:editorialNote "Cardinality: 0..1" .

linkml:specimen__histological_composition_measure a owl:ObjectProperty,
        linkml:SlotDefinition ;
    rdfs:label "specimen__histological_composition_measure" ;
    rdfs:range <https://example.org/ccdh/Observation> ;
    skos:definition "An observation that quantifies the relative or absolute composition of a specimen at cellular level, - i.e. how many cells in the specimen are of a given type, or exhibit a particular cellular phenotype. This information is typically determined through microscopic analysis of a slide." ;
    skos:editorialNote "Cardinality: 0..m" .

linkml:specimen__id a owl:ObjectProperty,
        linkml:SlotDefinition ;
    rdfs:label "specimen__id" ;
    rdfs:range <https://example.org/ccdh/CcdhString> ;
    skos:definition "The 'logical' identifier of the entity in the system of record.  This 'id' is guaranteed to be unique only within a given system, but not globally. The identified entity may have a different 'id' in a different system, and have many external business 'identifiers' associated with it." ;
    skos:editorialNote "Cardinality: 0..1" .

linkml:specimen__identifier a owl:ObjectProperty,
        linkml:SlotDefinition ;
    rdfs:label "specimen__identifier" ;
    rdfs:range <https://example.org/ccdh/Identifier> ;
    skos:definition "A 'business' identifier  or accession number for the entity, typically as provided by an external system or authority, that us globally unique and persists across implementing systems." ;
    skos:editorialNote "Cardinality: 0..m" .

linkml:specimen__morphlogy_assessment_method a owl:ObjectProperty,
        linkml:SlotDefinition ;
    rdfs:label "specimen__morphlogy_assessment_method" ;
    rdfs:range <http://UNKNOWN.org/enum_CRDC-H.Specimen.morphlogy_assessment_method> ;
    skos:definition "The general method used to assess a specimens specific tissue morphology" ;
    skos:editorialNote "Cardinality: 0..1" .

linkml:specimen__morphology_assessor_role a owl:ObjectProperty,
        linkml:SlotDefinition ;
    rdfs:label "specimen__morphology_assessor_role" ;
    rdfs:range <http://UNKNOWN.org/enum_CRDC-H.Specimen.morphology_assessor_role> ;
    skos:definition "A term describing the role of the person who histologically assessed the specific tissue morphology of a specimen" ;
    skos:editorialNote "Cardinality: 0..1" .

linkml:specimen__morphology_pathologically_confirmed a owl:ObjectProperty,
        linkml:SlotDefinition ;
    rdfs:label "specimen__morphology_pathologically_confirmed" ;
    rdfs:range <https://example.org/ccdh/CcdhBoolean> ;
    skos:definition "A flag indicating whether the histologic assessment of specific morphology was confirmed by a pathologist review" ;
    skos:editorialNote "Cardinality: 0..1" .

linkml:specimen__parent_specimen a owl:ObjectProperty,
        linkml:SlotDefinition ;
    rdfs:label "specimen__parent_specimen" ;
    rdfs:range <https://example.org/ccdh/Specimen> ;
    skos:definition "An existing specimen from which the specimen of interest was directly derived (i.e its immediate parent specimen)." ;
    skos:editorialNote "Cardinality: 0..m" .

linkml:specimen__preinvasive_tissue_morphology a owl:ObjectProperty,
        linkml:SlotDefinition ;
    rdfs:label "specimen__preinvasive_tissue_morphology" ;
    rdfs:range <http://UNKNOWN.org/enum_CRDC-H.Specimen.preinvasive_tissue_morphology> ;
    skos:definition "A term describing the pathology exhibited by a pre-invasive tissue in a specimen." ;
    skos:editorialNote "Cardinality: 0..1" .

linkml:specimen__processing_activity a owl:ObjectProperty,
        linkml:SlotDefinition ;
    rdfs:label "specimen__processing_activity" ;
    rdfs:range <https://example.org/ccdh/SpecimenProcessingActivity> ;
    skos:definition "An activity that modifies the physical structure, composition, or state of a specimen." ;
    skos:editorialNote "Cardinality: 0..m" .

linkml:specimen__quality_measure a owl:ObjectProperty,
        linkml:SlotDefinition ;
    rdfs:label "specimen__quality_measure" ;
    rdfs:range <https://example.org/ccdh/Observation> ;
    skos:definition "An observation about characteristics of a specimen that are indicative of its quality or suitability for use." ;
    skos:editorialNote "Cardinality: 0..m" .

linkml:specimen__quantity_measure a owl:ObjectProperty,
        linkml:SlotDefinition ;
    rdfs:label "specimen__quantity_measure" ;
    rdfs:range <https://example.org/ccdh/Observation> ;
    skos:definition "An observation related to the quantity of a specimen or analyte it currently contains - e.g. its weight, volume, or concentration." ;
    skos:editorialNote "Cardinality: 0..m" .

linkml:specimen__related_document a owl:ObjectProperty,
        linkml:SlotDefinition ;
    rdfs:label "specimen__related_document" ;
    rdfs:range <https://example.org/ccdh/Document> ;
    skos:definition "A reference to an external document that is about or related to the specimen (e.g. a publication related to the study it is a part of, pathology report containing additional details about it, protocol describing how it was collected, or a catalog entry describing  related research resource)" ;
    skos:editorialNote "Cardinality: 0..m" .

linkml:specimen__section_location a owl:ObjectProperty,
        linkml:SlotDefinition ;
    rdfs:label "specimen__section_location" ;
    rdfs:range <http://UNKNOWN.org/enum_CRDC-H.Specimen.section_location> ;
    skos:definition "The location in a parent specimen from which a section/portion was excised (e.g. top, middle, bottom)" ;
    skos:editorialNote "Cardinality: 0..1" .

linkml:specimen__source_material_type a owl:ObjectProperty,
        linkml:SlotDefinition ;
    rdfs:label "specimen__source_material_type" ;
    rdfs:range <http://UNKNOWN.org/enum_CRDC-H.Specimen.source_material_type> ;
    skos:definition "The general kind of material from which the specimen was derived, based on the physical nature of the source material." ;
    skos:editorialNote "Cardinality: 0..1" .

linkml:specimen__source_model_system a owl:ObjectProperty,
        linkml:SlotDefinition ;
    rdfs:label "specimen__source_model_system" ;
    rdfs:range <https://example.org/ccdh/Entity> ;
    skos:definition "A model biological system (e.g. a cell line, tissue culture, organoid) from which a specimen was directly or indirectly derived." ;
    skos:editorialNote "Cardinality: 0..1" .

linkml:specimen__source_subject a owl:ObjectProperty,
        linkml:SlotDefinition ;
    rdfs:label "specimen__source_subject" ;
    rdfs:range <https://example.org/ccdh/Subject> ;
    skos:definition "A Subject from which the specimen was directly or indirectly derived." ;
    skos:editorialNote "Cardinality: 0..1" .

linkml:specimen__specific_tissue_morphology a owl:ObjectProperty,
        linkml:SlotDefinition ;
    rdfs:label "specimen__specific_tissue_morphology" ;
    rdfs:range <http://UNKNOWN.org/enum_CRDC-H.Specimen.specific_tissue_morphology> ;
    skos:definition "A term describing the specific pathology exhibited by the tissue in a specimen." ;
    skos:editorialNote "Cardinality: 0..1" .

linkml:specimen__specimen_type a owl:ObjectProperty,
        linkml:SlotDefinition ;
    rdfs:label "specimen__specimen_type" ;
    rdfs:range <http://UNKNOWN.org/enum_CRDC-H.Specimen.specimen_type> ;
    skos:definition "The high-level type of the specimen, based on its derivation provenance (i.e. how far removed it is from the original sample extracted from a source)." ;
    skos:editorialNote "Cardinality: 0..1" .

linkml:specimen__storage_activity a owl:ObjectProperty,
        linkml:SlotDefinition ;
    rdfs:label "specimen__storage_activity" ;
    rdfs:range <https://example.org/ccdh/SpecimenStorageActivity> ;
    skos:definition "An activity that results in the storage or maintenance of a specimen in a particular location, container, or state." ;
    skos:editorialNote "Cardinality: 0..1" .

linkml:specimen__transport_activity a owl:ObjectProperty,
        linkml:SlotDefinition ;
    rdfs:label "specimen__transport_activity" ;
    rdfs:range <https://example.org/ccdh/SpecimenTransportActivity> ;
    skos:definition "An activity through which the specimen is transported between locations." ;
    skos:editorialNote "Cardinality: 0..1" .

linkml:specimen__tumor_status_at_collection a owl:ObjectProperty,
        linkml:SlotDefinition ;
    rdfs:label "specimen__tumor_status_at_collection" ;
    rdfs:range <http://UNKNOWN.org/enum_CRDC-H.Specimen.tumor_status_at_collection> ;
    skos:definition "The status of the tumor at the time the specimen was collected (e.g. if it was primary, recurrent, metastatic, etc)." ;
    skos:editorialNote "Cardinality: 0..1" .

linkml:subject__age_at_death a owl:ObjectProperty,
        linkml:SlotDefinition ;
    rdfs:label "subject__age_at_death" ;
    rdfs:range <https://example.org/ccdh/Quantity> ;
    skos:definition "The age of an individual at the time of death, expressed in days since birth" ;
    skos:editorialNote "Cardinality: 0..1" .

linkml:subject__breed a owl:ObjectProperty,
        linkml:SlotDefinition ;
    rdfs:label "subject__breed" ;
    rdfs:range <http://UNKNOWN.org/enum_CRDC-H.Subject.breed> ;
    skos:definition "A label given to a group of animals homogeneous in appearance and other characteristics that distinguish it from other animals of the same species." ;
    skos:editorialNote "Cardinality: 0..1" .

linkml:subject__cause_of_death a owl:ObjectProperty,
        linkml:SlotDefinition ;
    rdfs:label "subject__cause_of_death" ;
    rdfs:range <http://UNKNOWN.org/enum_CRDC-H.Subject.cause_of_death> ;
    skos:definition "Coded value indicating the circumstance or condition that results in the death of the subject." ;
    skos:editorialNote "Cardinality: 0..1" .

linkml:subject__ethnicity a owl:ObjectProperty,
        linkml:SlotDefinition ;
    rdfs:label "subject__ethnicity" ;
    rdfs:range <http://UNKNOWN.org/enum_CRDC-H.Subject.ethnicity> ;
    skos:definition """An individual's self-described social and cultural grouping, specifically whether an individual describes themselves as Hispanic or Latino. The provided values are based on the categories defined by the U.S. Office of Management and Business and used by the U.S. Census Bureau.

Applicable only when Subject.species is Homo Sapiens""" ;
    skos:editorialNote "Cardinality: 0..1" .

linkml:subject__id a owl:ObjectProperty,
        linkml:SlotDefinition ;
    rdfs:label "subject__id" ;
    rdfs:range <https://example.org/ccdh/CcdhString> ;
    skos:definition "The 'logical' identifier of the entity in the system of record.  This 'id' is guaranteed to be unique only within a given system, but not globally. The identified entity may have a different 'id' in a different system, and have many external business 'identifiers' associated with it." ;
    skos:editorialNote "Cardinality: 1..1" .

linkml:subject__identifier a owl:ObjectProperty,
        linkml:SlotDefinition ;
    rdfs:label "subject__identifier" ;
    rdfs:range <https://example.org/ccdh/Identifier> ;
    skos:definition "A 'business' identifier for the entity, typically as provided by an external system or authority, that persists across implementing systems." ;
    skos:editorialNote "Cardinality: 0..m" .

linkml:subject__race a owl:ObjectProperty,
        linkml:SlotDefinition ;
    rdfs:label "subject__race" ;
    rdfs:range <http://UNKNOWN.org/enum_CRDC-H.Subject.race> ;
    skos:definition """An arbitrary classification of a taxonomic group that is a division of a species. It usually arises as a consequence of geographical isolation within a species and is characterized by shared heredity, physical attributes and behavior, and in the case of humans, by common history, nationality, or geographic distribution. The provided values are based on the categories defined by the U.S. Office of Management and Business and used by the U.S. Census Bureau.

Applicable only when Subject.species is Homo Sapiens""" ;
    skos:editorialNote "Cardinality: 0..m" .

linkml:subject__sex a owl:ObjectProperty,
        linkml:SlotDefinition ;
    rdfs:label "subject__sex" ;
    rdfs:range <http://UNKNOWN.org/enum_CRDC-H.Subject.sex> ;
    skos:definition "The biologic character or quality that distinguishes male and female from one another as expressed by analysis of the person's gonadal, morphologic (internal and external), chromosomal, and hormonal characteristics." ;
    skos:editorialNote "Cardinality: 0..1" .

linkml:subject__species a owl:ObjectProperty,
        linkml:SlotDefinition ;
    rdfs:label "subject__species" ;
    rdfs:range <http://UNKNOWN.org/enum_CRDC-H.Subject.species> ;
    skos:definition "The scientific binomial name for the species of the subject (e.g. Homo sapiens, Mus musculus, etc.)" ;
    skos:editorialNote "Cardinality: 0..1" .

linkml:subject__vital_status a owl:ObjectProperty,
        linkml:SlotDefinition ;
    rdfs:label "subject__vital_status" ;
    rdfs:range <http://UNKNOWN.org/enum_CRDC-H.Subject.vital_status> ;
    skos:definition "Coded value indicating the state or condition of being living or deceased; also includes the case where the vital status is unknown." ;
    skos:editorialNote "Cardinality: 0..1" .

linkml:subject__year_of_birth a owl:ObjectProperty,
        linkml:SlotDefinition ;
    rdfs:label "subject__year_of_birth" ;
    rdfs:range <https://example.org/ccdh/CcdhInteger> ;
    skos:definition "Numeric value to represent the calendar year in which an individual was born." ;
    skos:editorialNote "Cardinality: 0..1" .

linkml:subject__year_of_death a owl:ObjectProperty,
        linkml:SlotDefinition ;
    rdfs:label "subject__year_of_death" ;
    rdfs:range <https://example.org/ccdh/CcdhInteger> ;
    skos:definition "Numeric value to represent the calendar year in which an individual died." ;
    skos:editorialNote "Cardinality: 0..1" .

linkml:substance__role a owl:ObjectProperty,
        linkml:SlotDefinition ;
    rdfs:label "substance__role" ;
    rdfs:range <http://UNKNOWN.org/enum_CRDC-H.Substance.role> ;
    skos:definition "A role played by the subtance in a particular applicaton (e.g. the role of a lysis buffer when applied in a specimen creation activity, or the role of fixative when applied in specimen processing)" ;
    skos:editorialNote "Cardinality: 0..m" .

linkml:substance__substance_type a owl:ObjectProperty,
        linkml:SlotDefinition ;
    rdfs:label "substance__substance_type" ;
    rdfs:range <http://UNKNOWN.org/enum_CRDC-H.Substance.substance_type> ;
    skos:definition "The specific type of the substance - at as granular a level as possible. May be a specific chemical compound, or the name of a formulation/preparation made up of many compounds." ;
    skos:editorialNote "Cardinality: 0..1" .

linkml:timePeriod__periodEnd_end a owl:ObjectProperty,
        linkml:SlotDefinition ;
    rdfs:label "timePeriod__periodEnd_end" ;
    rdfs:range <https://example.org/ccdh/TimePoint> ;
    skos:definition "When a period of time ended." ;
    skos:editorialNote "Cardinality: 0..1" .

linkml:timePeriod__periodStart_start a owl:ObjectProperty,
        linkml:SlotDefinition ;
    rdfs:label "timePeriod__periodStart_start" ;
    rdfs:range <https://example.org/ccdh/TimePoint> ;
    skos:definition "When a period of time started." ;
    skos:editorialNote "Cardinality: 0..1" .

linkml:timePoint__dateTime a owl:ObjectProperty,
        linkml:SlotDefinition ;
    rdfs:label "timePoint__dateTime" ;
    rdfs:range <https://example.org/ccdh/CcdhDateTime> ;
    skos:definition "An explicitly specified timepoint described in terms of a date and optionally a time on that date." ;
    skos:editorialNote "Cardinality: 0..1" .

linkml:timePoint__indexDate a owl:ObjectProperty,
        linkml:SlotDefinition ;
    rdfs:label "timePoint__indexDate" ;
    rdfs:range <https://example.org/ccdh/CcdhDateTime> ;
    skos:definition "An explicit dateTime that serves as a reference against which a specified offset compared to derive a specific timepoint." ;
    skos:editorialNote "Cardinality: 0..1" .

linkml:timePoint__indexEventType a owl:ObjectProperty,
        linkml:SlotDefinition ;
    rdfs:label "timePoint__indexEventType" ;
    rdfs:range <http://UNKNOWN.org/enum_CRDC-H.TimePoint.indexEventType> ;
    skos:definition "A type of event that is associated with a specific date, and which serves as a reference against which a specified offset compared to derive a specific timepoint." ;
    skos:editorialNote "Cardinality: 0..1" .

linkml:timePoint__offsetFromIndex a owl:ObjectProperty,
        linkml:SlotDefinition ;
    rdfs:label "timePoint__offsetFromIndex" ;
    rdfs:range <https://example.org/ccdh/Quantity> ;
    skos:definition "A quantity of time that, together with the index date or event, can be used to derive a specific timepoint." ;
    skos:editorialNote "Cardinality: 0..1" .

linkml:treatment__anatomic_site a owl:ObjectProperty,
        linkml:SlotDefinition ;
    rdfs:label "treatment__anatomic_site" ;
    rdfs:range <https://example.org/ccdh/BodySite> ;
    skos:definition "The anatomical site that the treatment targets." ;
    skos:editorialNote "Cardinality: 0..1" .

linkml:treatment__concurrent_treatment a owl:ObjectProperty,
        linkml:SlotDefinition ;
    rdfs:label "treatment__concurrent_treatment" ;
    rdfs:range <https://example.org/ccdh/Treatment> ;
    skos:definition "The treatment(s) instance(s) that are concurrent with this treatment." ;
    skos:editorialNote "Cardinality: 0..m" .

linkml:treatment__concurrent_treatment_type a owl:ObjectProperty,
        linkml:SlotDefinition ;
    rdfs:label "treatment__concurrent_treatment_type" ;
    rdfs:range <https://example.org/ccdh/CcdhString> ;
    skos:definition "The type(s) of treatment(s) that are concurrent to this treatment." ;
    skos:editorialNote "Cardinality: 0..m" .

linkml:treatment__diagnosis a owl:ObjectProperty,
        linkml:SlotDefinition ;
    rdfs:label "treatment__diagnosis" ;
    rdfs:range <https://example.org/ccdh/Diagnosis> ;
    skos:definition "The diagnosis for which this treatement is intended for" ;
    skos:editorialNote "Cardinality: 0..m" .

linkml:treatment__effect a owl:ObjectProperty,
        linkml:SlotDefinition ;
    rdfs:label "treatment__effect" ;
    rdfs:range <https://example.org/ccdh/CcdhString> ;
    skos:definition "The effect of a treatment on the diagnosis or tumor." ;
    skos:editorialNote "Cardinality: 0..1" .

linkml:treatment__end_date a owl:ObjectProperty,
        linkml:SlotDefinition ;
    rdfs:label "treatment__end_date" ;
    rdfs:range <https://example.org/ccdh/TimePoint> ;
    skos:definition "The timepoint at which the treatment ended." ;
    skos:editorialNote "Cardinality: 0..1" .

linkml:treatment__end_reason a owl:ObjectProperty,
        linkml:SlotDefinition ;
    rdfs:label "treatment__end_reason" ;
    rdfs:range <https://example.org/ccdh/CcdhString> ;
    skos:definition "" .

linkml:treatment__id a owl:ObjectProperty,
        linkml:SlotDefinition ;
    rdfs:label "treatment__id" ;
    rdfs:range <https://example.org/ccdh/CcdhString> ;
    skos:definition "" ;
    skos:editorialNote "Cardinality: 0..1" .

linkml:treatment__identifier a owl:ObjectProperty,
        linkml:SlotDefinition ;
    rdfs:label "treatment__identifier" ;
    rdfs:range <https://example.org/ccdh/Identifier> ;
    skos:definition "The regimen or line of therapy" ;
    skos:editorialNote "Cardinality: 0..m" .

linkml:treatment__intent a owl:ObjectProperty,
        linkml:SlotDefinition ;
    rdfs:label "treatment__intent" ;
    rdfs:range <https://example.org/ccdh/CcdhString> ;
    skos:definition "The intent of the treatment." ;
    skos:editorialNote "Cardinality: 0..1" .

linkml:treatment__number_of_cycles a owl:ObjectProperty,
        linkml:SlotDefinition ;
    rdfs:label "treatment__number_of_cycles" ;
    rdfs:range <https://example.org/ccdh/CcdhInteger> ;
    skos:definition "The number of treatment cycles the patient received." ;
    skos:editorialNote "Cardinality: 0..1" .

linkml:treatment__outcome a owl:ObjectProperty,
        linkml:SlotDefinition ;
    rdfs:label "treatment__outcome" ;
    rdfs:range <https://example.org/ccdh/CcdhString> ;
    skos:definition "The final outcome of the treatment." ;
    skos:editorialNote "Cardinality: 0..1" .

linkml:treatment__regimen a owl:ObjectProperty,
        linkml:SlotDefinition ;
    rdfs:label "treatment__regimen" ;
    rdfs:range <https://example.org/ccdh/CcdhString> ;
    skos:definition "" ;
    skos:editorialNote "Cardinality: 0..1" .

linkml:treatment__start_date a owl:ObjectProperty,
        linkml:SlotDefinition ;
    rdfs:label "treatment__start_date" ;
    rdfs:range <https://example.org/ccdh/TimePoint> ;
    skos:definition "The timepoint at which the treatment started." ;
    skos:editorialNote "Cardinality: 0..1" .

linkml:treatment__therapeutic_agent a owl:ObjectProperty,
        linkml:SlotDefinition ;
    rdfs:label "treatment__therapeutic_agent" ;
    rdfs:range <https://example.org/ccdh/Substance> ;
    skos:definition "One or more theraputic agents as part of this treatment." ;
    skos:editorialNote "Cardinality: 0..m" .

linkml:treatment__type a owl:ObjectProperty,
        linkml:SlotDefinition ;
    rdfs:label "treatment__type" ;
    rdfs:range <http://UNKNOWN.org/enum_CRDC-H.Treatment.type> ;
    skos:definition "The treatment type including medication/theraputics or other procedures." ;
    skos:editorialNote "Cardinality: 0..1" .

linkml:Boolean a owl:Class,
        linkml:TypeDefinition ;
    rdfs:label "boolean" ;
    rdfs:subClassOf [ a owl:Restriction ;
            owl:onDataRange xsd:boolean ;
            owl:onProperty linkml:topValue ;
            owl:qualifiedCardinality 1 ] ;
    skos:definition "A binary (true or false) value" .

linkml:Datetime a owl:Class,
        linkml:TypeDefinition ;
    rdfs:label "datetime" ;
    rdfs:subClassOf [ a owl:Restriction ;
            owl:onDataRange xsd:dateTime ;
            owl:onProperty linkml:topValue ;
            owl:qualifiedCardinality 1 ] ;
    skos:definition "The combination of a date and time" .

linkml:Decimal a owl:Class,
        linkml:TypeDefinition ;
    rdfs:label "decimal" ;
    rdfs:subClassOf [ a owl:Restriction ;
            owl:onDataRange xsd:decimal ;
            owl:onProperty linkml:topValue ;
            owl:qualifiedCardinality 1 ] ;
    skos:definition "A real number with arbitrary precision that conforms to the xsd:decimal specification" .

linkml:Integer a owl:Class,
        linkml:TypeDefinition ;
    rdfs:label "integer" ;
    rdfs:subClassOf [ a owl:Restriction ;
            owl:onDataRange xsd:integer ;
            owl:onProperty linkml:topValue ;
            owl:qualifiedCardinality 1 ] ;
    skos:definition "An integer" .

linkml:Uriorcurie a owl:Class,
        linkml:TypeDefinition ;
    rdfs:label "uriorcurie" ;
    rdfs:subClassOf [ a owl:Restriction ;
            owl:onDataRange xsd:anyURI ;
            owl:onProperty linkml:topValue ;
            owl:qualifiedCardinality 1 ] ;
    skos:definition "a URI or a CURIE" .

<https://example.org/ccdh/BiologicProduct> a owl:Class,
        linkml:ClassDefinition ;
    rdfs:label "BiologicProduct" ;
    rdfs:subClassOf [ a owl:Restriction ;
            owl:maxQualifiedCardinality 1 ;
            owl:onClass <http://UNKNOWN.org/enum_CRDC-H.BiologicProduct.product_type> ;
            owl:onProperty linkml:product_type ],
        [ a owl:Restriction ;
            owl:allValuesFrom <https://example.org/ccdh/Identifier> ;
            owl:onProperty linkml:identifier ],
        [ a owl:Restriction ;
            owl:maxQualifiedCardinality 1 ;
            owl:onClass <https://example.org/ccdh/CcdhString> ;
            owl:onProperty linkml:id ],
        [ a owl:Restriction ;
            owl:allValuesFrom <https://example.org/ccdh/CcdhInteger> ;
            owl:onProperty linkml:passage_number ],
        [ a owl:Restriction ;
            owl:maxQualifiedCardinality 1 ;
            owl:onClass <https://example.org/ccdh/CcdhString> ;
            owl:onProperty linkml:description ],
        [ a owl:Restriction ;
            owl:allValuesFrom <https://example.org/ccdh/CcdhString> ;
            owl:onProperty linkml:growth_rate ],
        <https://example.org/ccdh/Entity> ;
    skos:definition "A living organism, or a metabolocally active biological system such as a cell culture, tissue culture, or organoid that is maintained or propagated in vitro." ;
    skos:editorialNote "Derived from [BiologicProduct in sheet BiologicProduct](https://docs.google.com/spreadsheets/d/1oWS7cao-fgz2MKWtyr8h2dEL9unX__0bJrWKv6mQmM4/edit#gid=1097989080)" .

<https://example.org/ccdh/CancerStageObservation> a owl:Class,
        linkml:ClassDefinition ;
    rdfs:label "CancerStageObservation" ;
    rdfs:subClassOf [ a owl:Restriction ;
            owl:maxQualifiedCardinality 1 ;
            owl:onClass <http://UNKNOWN.org/enum_CRDC-H.CancerStageObservation.valueCodeableConcept> ;
            owl:onProperty linkml:valueCodeableConcept ],
        [ a owl:Restriction ;
            owl:onClass <http://UNKNOWN.org/enum_CRDC-H.CancerStageObservation.observation_type> ;
            owl:onProperty linkml:observation_type ;
            owl:qualifiedCardinality 1 ],
        <https://example.org/ccdh/Entity> ;
    skos:definition "A data structure with key (observation_type) and value (valueCodeableConcept) attributes that represents a single cancer staging observation, such as the Clinical Metastasis (M) component of a clinical TNM staging." ;
    skos:editorialNote "Derived from [CancerStageObservation in sheet CancerStageObservation](https://docs.google.com/spreadsheets/d/1oWS7cao-fgz2MKWtyr8h2dEL9unX__0bJrWKv6mQmM4/edit#gid=2055385865)" .

<https://example.org/ccdh/CancerStageObservationSet> a owl:Class,
        linkml:ClassDefinition ;
    rdfs:label "CancerStageObservationSet" ;
    rdfs:subClassOf [ a owl:Restriction ;
            owl:allValuesFrom <https://example.org/ccdh/CancerStageObservation> ;
            owl:onProperty linkml:observations ],
        [ a owl:Restriction ;
            owl:maxQualifiedCardinality 1 ;
            owl:onClass <http://UNKNOWN.org/enum_CRDC-H.CancerStageObservationSet.method_type> ;
            owl:onProperty linkml:method_type ],
        [ a owl:Restriction ;
            owl:onClass <http://UNKNOWN.org/enum_CRDC-H.CancerStageObservationSet.category> ;
            owl:onProperty linkml:category ;
            owl:qualifiedCardinality 1 ],
        <https://example.org/ccdh/Entity> ;
    skos:definition "A structured object to hold related data items about the staging of cancer (e.g. overall, T, N, and M components of a Cancer Staging observation)." ;
    skos:editorialNote "Derived from [CancerStageObservationSet in sheet CancerStageObservationSet](https://docs.google.com/spreadsheets/d/1oWS7cao-fgz2MKWtyr8h2dEL9unX__0bJrWKv6mQmM4/edit#gid=985251464)" .

<https://example.org/ccdh/Document> a owl:Class,
        linkml:ClassDefinition ;
    rdfs:label "Document" ;
    rdfs:subClassOf [ a owl:Restriction ;
            owl:allValuesFrom <https://example.org/ccdh/CcdhString> ;
            owl:onProperty linkml:url ],
        [ a owl:Restriction ;
            owl:allValuesFrom <https://example.org/ccdh/Identifier> ;
            owl:onProperty linkml:identifier ],
        [ a owl:Restriction ;
            owl:maxQualifiedCardinality 1 ;
            owl:onClass <https://example.org/ccdh/Entity> ;
            owl:onProperty linkml:focus ],
        [ a owl:Restriction ;
            owl:maxQualifiedCardinality 1 ;
            owl:onClass <https://example.org/ccdh/CcdhString> ;
            owl:onProperty linkml:id ],
        [ a owl:Restriction ;
            owl:maxQualifiedCardinality 1 ;
            owl:onClass <http://UNKNOWN.org/enum_CRDC-H.Document.document_type> ;
            owl:onProperty linkml:document_type ],
        [ a owl:Restriction ;
            owl:maxQualifiedCardinality 1 ;
            owl:onClass <https://example.org/ccdh/CcdhString> ;
            owl:onProperty linkml:description ],
        <https://example.org/ccdh/Entity> ;
    skos:definition "" ;
    skos:editorialNote "Derived from [Document in sheet Document](https://docs.google.com/spreadsheets/d/1oWS7cao-fgz2MKWtyr8h2dEL9unX__0bJrWKv6mQmM4/edit#gid=809861603)" .

<https://example.org/ccdh/SpecimenCreationActivity> a owl:Class,
        linkml:ClassDefinition ;
    rdfs:label "SpecimenCreationActivity" ;
    rdfs:subClassOf [ a owl:Restriction ;
            owl:allValuesFrom <https://example.org/ccdh/Observation> ;
            owl:onProperty linkml:execution_observation ],
        [ a owl:Restriction ;
            owl:maxQualifiedCardinality 1 ;
            owl:onClass <http://UNKNOWN.org/enum_CRDC-H.SpecimenCreationActivity.derivation_method_type> ;
            owl:onProperty linkml:derivation_method_type ],
        [ a owl:Restriction ;
            owl:maxQualifiedCardinality 1 ;
            owl:onClass <https://example.org/ccdh/Quantity> ;
            owl:onProperty linkml:quantity_collected ],
        [ a owl:Restriction ;
            owl:maxQualifiedCardinality 1 ;
            owl:onClass <http://UNKNOWN.org/enum_CRDC-H.SpecimenCreationActivity.collection_method_type> ;
            owl:onProperty linkml:collection_method_type ],
        [ a owl:Restriction ;
            owl:maxQualifiedCardinality 1 ;
            owl:onClass <https://example.org/ccdh/TimePoint> ;
            owl:onProperty linkml:date_ended ],
        [ a owl:Restriction ;
            owl:maxQualifiedCardinality 1 ;
            owl:onClass <https://example.org/ccdh/CcdhString> ;
            owl:onProperty linkml:specimen_order ],
        [ a owl:Restriction ;
            owl:allValuesFrom <https://example.org/ccdh/Substance> ;
            owl:onProperty linkml:additive ],
        [ a owl:Restriction ;
            owl:maxQualifiedCardinality 1 ;
            owl:onClass <https://example.org/ccdh/Organization> ;
            owl:onProperty linkml:performed_by ],
        [ a owl:Restriction ;
            owl:maxQualifiedCardinality 1 ;
            owl:onClass <http://UNKNOWN.org/enum_CRDC-H.SpecimenCreationActivity.activity_type> ;
            owl:onProperty linkml:activity_type ],
        [ a owl:Restriction ;
            owl:allValuesFrom <https://example.org/ccdh/Specimen> ;
            owl:onProperty linkml:input_specimen ],
        [ a owl:Restriction ;
            owl:maxQualifiedCardinality 1 ;
            owl:onClass <https://example.org/ccdh/BodySite> ;
            owl:onProperty linkml:collection_site ],
        [ a owl:Restriction ;
            owl:maxQualifiedCardinality 1 ;
            owl:onClass <https://example.org/ccdh/TimePoint> ;
            owl:onProperty linkml:date_started ],
        <https://example.org/ccdh/Entity> ;
    skos:definition "The process of creating a specimen through observing and/or removing material from an biological source or natural setting (e.g. from a person, animal, cell line, or environmental material), or through derivation from an existing specimen (e.g. through portioning or aliquoting). This activity represents the entire process up to the point where the specimen is physically modified, stored, or transported." ;
    skos:editorialNote "Derived from [SpecimenCreationActivity in sheet SpecimenCreationActivity](https://docs.google.com/spreadsheets/d/1oWS7cao-fgz2MKWtyr8h2dEL9unX__0bJrWKv6mQmM4/edit#gid=693792130)" .

<https://example.org/ccdh/SpecimenProcessingActivity> a owl:Class,
        linkml:ClassDefinition ;
    rdfs:label "SpecimenProcessingActivity" ;
    rdfs:subClassOf [ a owl:Restriction ;
            owl:maxQualifiedCardinality 1 ;
            owl:onClass <https://example.org/ccdh/Organization> ;
            owl:onProperty linkml:performed_by ],
        [ a owl:Restriction ;
            owl:allValuesFrom <https://example.org/ccdh/Entity> ;
            owl:onProperty linkml:execution_observation ],
        [ a owl:Restriction ;
            owl:allValuesFrom <https://example.org/ccdh/Substance> ;
            owl:onProperty linkml:additive ],
        [ a owl:Restriction ;
            owl:maxQualifiedCardinality 1 ;
            owl:onClass <http://UNKNOWN.org/enum_CRDC-H.SpecimenProcessingActivity.activity_type> ;
            owl:onProperty linkml:activity_type ],
        [ a owl:Restriction ;
            owl:maxQualifiedCardinality 1 ;
            owl:onClass <https://example.org/ccdh/TimePoint> ;
            owl:onProperty linkml:date_ended ],
        [ a owl:Restriction ;
            owl:maxQualifiedCardinality 1 ;
            owl:onClass <https://example.org/ccdh/TimePoint> ;
            owl:onProperty linkml:date_started ],
        [ a owl:Restriction ;
            owl:maxQualifiedCardinality 1 ;
            owl:onClass <http://UNKNOWN.org/enum_CRDC-H.SpecimenProcessingActivity.method_type> ;
            owl:onProperty linkml:method_type ],
        [ a owl:Restriction ;
            owl:allValuesFrom <https://example.org/ccdh/Entity> ;
            owl:onProperty linkml:duration ],
        <https://example.org/ccdh/Entity> ;
    skos:definition "An activity that modifies the physical structure, composition, or state of a specimen. Unlike SpecimenCreation, SpecimenProcessing activities do not result in the generation of new entities - they take a single specimen as input, and output that same specimen." ;
    skos:editorialNote "Derived from [SpecimenProcessingActivity in sheet SpecimenProcessingActivity](https://docs.google.com/spreadsheets/d/1oWS7cao-fgz2MKWtyr8h2dEL9unX__0bJrWKv6mQmM4/edit#gid=1726416617)" .

<https://example.org/ccdh/SpecimenStorageActivity> a owl:Class,
        linkml:ClassDefinition ;
    rdfs:label "SpecimenStorageActivity" ;
    rdfs:subClassOf [ a owl:Restriction ;
            owl:maxQualifiedCardinality 1 ;
            owl:onClass <https://example.org/ccdh/TimePoint> ;
            owl:onProperty linkml:date_started ],
        [ a owl:Restriction ;
            owl:maxQualifiedCardinality 1 ;
            owl:onClass <https://example.org/ccdh/TimePoint> ;
            owl:onProperty linkml:date_ended ],
        [ a owl:Restriction ;
            owl:maxQualifiedCardinality 1 ;
            owl:onClass <http://UNKNOWN.org/enum_CRDC-H.SpecimenStorageActivity.method_type> ;
            owl:onProperty linkml:method_type ],
        [ a owl:Restriction ;
            owl:allValuesFrom <https://example.org/ccdh/SpecimenContainer> ;
            owl:onProperty linkml:container ],
        [ a owl:Restriction ;
            owl:maxQualifiedCardinality 1 ;
            owl:onClass <https://example.org/ccdh/Organization> ;
            owl:onProperty linkml:performed_by ],
        [ a owl:Restriction ;
            owl:maxQualifiedCardinality 1 ;
            owl:onClass <https://example.org/ccdh/Quantity> ;
            owl:onProperty linkml:duration ],
        <https://example.org/ccdh/Entity> ;
    skos:definition """An activity in which a specimen is stored or maintained in a particular location, container, or state. Unlike 'processing' activities, storage does not alter the 
intrinsic physical nature of a specimen.""" ;
    skos:editorialNote "Derived from [SpecimenStorageActivity in sheet SpecimenStorageActivity](https://docs.google.com/spreadsheets/d/1oWS7cao-fgz2MKWtyr8h2dEL9unX__0bJrWKv6mQmM4/edit#gid=1583133214)" .

<https://example.org/ccdh/SpecimenTransportActivity> a owl:Class,
        linkml:ClassDefinition ;
    rdfs:label "SpecimenTransportActivity" ;
    rdfs:subClassOf [ a owl:Restriction ;
            owl:maxQualifiedCardinality 1 ;
            owl:onClass <https://example.org/ccdh/Organization> ;
            owl:onProperty linkml:transport_origin ],
        [ a owl:Restriction ;
            owl:allValuesFrom <https://example.org/ccdh/CcdhString> ;
            owl:onProperty linkml:duration ],
        [ a owl:Restriction ;
            owl:allValuesFrom <https://example.org/ccdh/Entity> ;
            owl:onProperty linkml:execution_observation ],
        [ a owl:Restriction ;
            owl:maxQualifiedCardinality 1 ;
            owl:onClass <https://example.org/ccdh/Organization> ;
            owl:onProperty linkml:transport_destination ],
        [ a owl:Restriction ;
            owl:maxQualifiedCardinality 1 ;
            owl:onClass <https://example.org/ccdh/Organization> ;
            owl:onProperty linkml:performed_by ],
        [ a owl:Restriction ;
            owl:maxQualifiedCardinality 1 ;
            owl:onClass <https://example.org/ccdh/TimePoint> ;
            owl:onProperty linkml:date_ended ],
        [ a owl:Restriction ;
            owl:allValuesFrom <https://example.org/ccdh/CcdhString> ;
            owl:onProperty linkml:execution_conditions ],
        [ a owl:Restriction ;
            owl:maxQualifiedCardinality 1 ;
            owl:onClass <https://example.org/ccdh/TimePoint> ;
            owl:onProperty linkml:date_started ],
        <https://example.org/ccdh/Entity> ;
    skos:definition "An activity through which a specimen is transported between locations." ;
    skos:editorialNote "Derived from [SpecimenTransportActivity in sheet SpecimenTransportActivity](https://docs.google.com/spreadsheets/d/1oWS7cao-fgz2MKWtyr8h2dEL9unX__0bJrWKv6mQmM4/edit#gid=359352096)" .

<https://example.org/ccdh/Treatment> a owl:Class,
        linkml:ClassDefinition ;
    rdfs:label "Treatment" ;
    rdfs:subClassOf [ a owl:Restriction ;
            owl:maxQualifiedCardinality 1 ;
            owl:onClass <https://example.org/ccdh/TimePoint> ;
            owl:onProperty linkml:start_date ],
        [ a owl:Restriction ;
            owl:allValuesFrom <https://example.org/ccdh/Diagnosis> ;
            owl:onProperty linkml:diagnosis ],
        [ a owl:Restriction ;
            owl:allValuesFrom <https://example.org/ccdh/CcdhString> ;
            owl:onProperty linkml:end_reason ],
        [ a owl:Restriction ;
            owl:maxQualifiedCardinality 1 ;
            owl:onClass <https://example.org/ccdh/BodySite> ;
            owl:onProperty linkml:anatomic_site ],
        [ a owl:Restriction ;
            owl:allValuesFrom <https://example.org/ccdh/Treatment> ;
            owl:onProperty linkml:concurrent_treatment ],
        [ a owl:Restriction ;
            owl:maxQualifiedCardinality 1 ;
            owl:onClass <https://example.org/ccdh/TimePoint> ;
            owl:onProperty linkml:end_date ],
        [ a owl:Restriction ;
            owl:maxQualifiedCardinality 1 ;
            owl:onClass <https://example.org/ccdh/CcdhString> ;
            owl:onProperty linkml:regimen ],
        [ a owl:Restriction ;
            owl:maxQualifiedCardinality 1 ;
            owl:onClass <https://example.org/ccdh/CcdhString> ;
            owl:onProperty linkml:id ],
        [ a owl:Restriction ;
            owl:maxQualifiedCardinality 1 ;
            owl:onClass <http://UNKNOWN.org/enum_CRDC-H.Treatment.type> ;
            owl:onProperty linkml:type ],
        [ a owl:Restriction ;
            owl:maxQualifiedCardinality 1 ;
            owl:onClass <https://example.org/ccdh/CcdhInteger> ;
            owl:onProperty linkml:number_of_cycles ],
        [ a owl:Restriction ;
            owl:maxQualifiedCardinality 1 ;
            owl:onClass <https://example.org/ccdh/CcdhString> ;
            owl:onProperty linkml:outcome ],
        [ a owl:Restriction ;
            owl:allValuesFrom <https://example.org/ccdh/Identifier> ;
            owl:onProperty linkml:identifier ],
        [ a owl:Restriction ;
            owl:maxQualifiedCardinality 1 ;
            owl:onClass <https://example.org/ccdh/CcdhString> ;
            owl:onProperty linkml:effect ],
        [ a owl:Restriction ;
            owl:allValuesFrom <https://example.org/ccdh/Substance> ;
            owl:onProperty linkml:therapeutic_agent ],
        [ a owl:Restriction ;
            owl:allValuesFrom <https://example.org/ccdh/CcdhString> ;
            owl:onProperty linkml:concurrent_treatment_type ],
        [ a owl:Restriction ;
            owl:maxQualifiedCardinality 1 ;
            owl:onClass <https://example.org/ccdh/CcdhString> ;
            owl:onProperty linkml:intent ],
        <https://example.org/ccdh/Entity> ;
    skos:definition "Represent medication administration or other treatment types." ;
    skos:editorialNote "Derived from [Treatment in sheet Treatment](https://docs.google.com/spreadsheets/d/1oWS7cao-fgz2MKWtyr8h2dEL9unX__0bJrWKv6mQmM4/edit#gid=2111784779)" .

linkml:String a owl:Class,
        linkml:TypeDefinition ;
    rdfs:label "string" ;
    rdfs:subClassOf [ a owl:Restriction ;
            owl:onDataRange xsd:string ;
            owl:onProperty linkml:topValue ;
            owl:qualifiedCardinality 1 ] ;
    skos:definition "A character string" .

<https://example.org/ccdh/CcdhBoolean> a owl:Class,
        linkml:TypeDefinition ;
    rdfs:label "ccdh_boolean" ;
    rdfs:subClassOf linkml:Boolean ;
    skos:definition "Value representing either “true” or “false”.  Permissible values (case-sensitive) = “true”, “false”, “1”, “0”." ;
    skos:editorialNote "Derived from [ccdh_boolean in sheet Primitives](https://docs.google.com/spreadsheets/d/1oWS7cao-fgz2MKWtyr8h2dEL9unX__0bJrWKv6mQmM4/edit#gid=497370447)" .

<https://example.org/ccdh/CcdhDecimal> a owl:Class,
        linkml:TypeDefinition ;
    rdfs:label "ccdh_decimal" ;
    rdfs:subClassOf linkml:Decimal ;
    skos:definition "A rational number that has a decimal representation.  This data type does not restrict the size or precision of the number." ;
    skos:editorialNote "Derived from [ccdh_decimal in sheet Primitives](https://docs.google.com/spreadsheets/d/1oWS7cao-fgz2MKWtyr8h2dEL9unX__0bJrWKv6mQmM4/edit#gid=497370447)" .

<https://example.org/ccdh/Coding> a owl:Class,
        linkml:ClassDefinition ;
    rdfs:label "Coding" ;
    rdfs:subClassOf [ a owl:Restriction ;
            owl:onClass <https://example.org/ccdh/CcdhString> ;
            owl:onProperty linkml:code ;
            owl:qualifiedCardinality 1 ],
        [ a owl:Restriction ;
            owl:onClass <https://example.org/ccdh/CcdhString> ;
            owl:onProperty linkml:system ;
            owl:qualifiedCardinality 1 ],
        [ a owl:Restriction ;
            owl:maxQualifiedCardinality 1 ;
            owl:onClass <https://example.org/ccdh/CcdhString> ;
            owl:onProperty linkml:systemVersion ],
        [ a owl:Restriction ;
            owl:maxQualifiedCardinality 1 ;
            owl:onClass <https://example.org/ccdh/CcdhString> ;
            owl:onProperty linkml:systemURL ],
        [ a owl:Restriction ;
            owl:maxQualifiedCardinality 1 ;
            owl:onClass <https://example.org/ccdh/CcdhString> ;
            owl:onProperty linkml:label ],
        <https://example.org/ccdh/Entity> ;
    skos:definition "A structured representation of a coded/enumerated data value, that includes additional metadata about the code and code system." ;
    skos:editorialNote "Derived from [Coding in sheet Coding](https://docs.google.com/spreadsheets/d/1oWS7cao-fgz2MKWtyr8h2dEL9unX__0bJrWKv6mQmM4/edit#gid=1218588936)" .

<https://example.org/ccdh/ResearchProject> a owl:Class,
        linkml:ClassDefinition ;
    rdfs:label "ResearchProject" ;
    rdfs:subClassOf [ a owl:Restriction ;
            owl:maxQualifiedCardinality 1 ;
            owl:onClass <https://example.org/ccdh/CcdhString> ;
            owl:onProperty linkml:name_shortened ],
        [ a owl:Restriction ;
            owl:maxQualifiedCardinality 1 ;
            owl:onClass <https://example.org/ccdh/CcdhString> ;
            owl:onProperty linkml:name ],
        [ a owl:Restriction ;
            owl:maxQualifiedCardinality 1 ;
            owl:onClass <https://example.org/ccdh/CcdhDateTime> ;
            owl:onProperty linkml:date_ended ],
        [ a owl:Restriction ;
            owl:maxQualifiedCardinality 1 ;
            owl:onClass <https://example.org/ccdh/CcdhString> ;
            owl:onProperty linkml:description_shortened ],
        [ a owl:Restriction ;
            owl:maxQualifiedCardinality 1 ;
            owl:onClass <https://example.org/ccdh/CcdhDateTime> ;
            owl:onProperty linkml:date_iacuc_approval ],
        [ a owl:Restriction ;
            owl:allValuesFrom <https://example.org/ccdh/ResearchProject> ;
            owl:onProperty linkml:part_of ],
        [ a owl:Restriction ;
            owl:maxQualifiedCardinality 1 ;
            owl:onClass <https://example.org/ccdh/CcdhString> ;
            owl:onProperty linkml:description ],
        [ a owl:Restriction ;
            owl:allValuesFrom <https://example.org/ccdh/Identifier> ;
            owl:onProperty linkml:identifier ],
        [ a owl:Restriction ;
            owl:onClass <http://UNKNOWN.org/enum_CRDC-H.ResearchProject.research_project_type> ;
            owl:onProperty linkml:research_project_type ;
            owl:qualifiedCardinality 1 ],
        [ a owl:Restriction ;
            owl:maxQualifiedCardinality 1 ;
            owl:onClass <https://example.org/ccdh/CcdhString> ;
            owl:onProperty linkml:id ],
        [ a owl:Restriction ;
            owl:allValuesFrom <https://example.org/ccdh/CcdhString> ;
            owl:onProperty linkml:url ],
        [ a owl:Restriction ;
            owl:maxQualifiedCardinality 1 ;
            owl:onClass <https://example.org/ccdh/CcdhDateTime> ;
            owl:onProperty linkml:date_started ],
        [ a owl:Restriction ;
            owl:allValuesFrom <https://example.org/ccdh/CcdhString> ;
            owl:onProperty linkml:sponsor ],
        [ a owl:Restriction ;
            owl:allValuesFrom <http://UNKNOWN.org/enum_CRDC-H.ResearchProject.primary_anatomic_site> ;
            owl:onProperty linkml:primary_anatomic_site ],
        <https://example.org/ccdh/Entity> ;
    skos:definition """A process where a researcher or organization plans and then executes a series of steps intended to increase the field of healthcare-related knowledge. 
This includes studies of safety, efficacy, comparative effectiveness and other information about medications, devices, therapies and other interventional 
and investigative techniques. A ResearchProject involves the gathering of information about human or animal subjects.""" ;
    skos:editorialNote "Derived from [ResearchProject in sheet ResearchProject](https://docs.google.com/spreadsheets/d/1oWS7cao-fgz2MKWtyr8h2dEL9unX__0bJrWKv6mQmM4/edit#gid=1123416579)" .

<https://example.org/ccdh/Specimen> a owl:Class,
        linkml:ClassDefinition ;
    rdfs:label "Specimen" ;
    rdfs:subClassOf [ a owl:Restriction ;
            owl:maxQualifiedCardinality 1 ;
            owl:onClass <https://example.org/ccdh/Organization> ;
            owl:onProperty linkml:data_provider ],
        [ a owl:Restriction ;
            owl:maxQualifiedCardinality 1 ;
            owl:onClass <http://UNKNOWN.org/enum_CRDC-H.Specimen.section_location> ;
            owl:onProperty linkml:section_location ],
        [ a owl:Restriction ;
            owl:maxQualifiedCardinality 1 ;
            owl:onClass <http://UNKNOWN.org/enum_CRDC-H.Specimen.source_material_type> ;
            owl:onProperty linkml:source_material_type ],
        [ a owl:Restriction ;
            owl:maxQualifiedCardinality 1 ;
            owl:onClass <https://example.org/ccdh/SpecimenContainer> ;
            owl:onProperty linkml:contained_in ],
        [ a owl:Restriction ;
            owl:allValuesFrom <https://example.org/ccdh/Observation> ;
            owl:onProperty linkml:quality_measure ],
        [ a owl:Restriction ;
            owl:maxQualifiedCardinality 1 ;
            owl:onClass <https://example.org/ccdh/Entity> ;
            owl:onProperty linkml:dimensional_measure ],
        [ a owl:Restriction ;
            owl:maxQualifiedCardinality 1 ;
            owl:onClass <https://example.org/ccdh/Entity> ;
            owl:onProperty linkml:source_model_system ],
        [ a owl:Restriction ;
            owl:maxQualifiedCardinality 1 ;
            owl:onClass <http://UNKNOWN.org/enum_CRDC-H.Specimen.degree_of_dysplasia> ;
            owl:onProperty linkml:degree_of_dysplasia ],
        [ a owl:Restriction ;
            owl:maxQualifiedCardinality 1 ;
            owl:onClass <http://UNKNOWN.org/enum_CRDC-H.Specimen.analyte_type> ;
            owl:onProperty linkml:analyte_type ],
        [ a owl:Restriction ;
            owl:maxQualifiedCardinality 1 ;
            owl:onClass <https://example.org/ccdh/SpecimenCreationActivity> ;
            owl:onProperty linkml:creation_activity ],
        [ a owl:Restriction ;
            owl:maxQualifiedCardinality 1 ;
            owl:onClass <https://example.org/ccdh/ResearchProject> ;
            owl:onProperty linkml:associated_project ],
        [ a owl:Restriction ;
            owl:maxQualifiedCardinality 1 ;
            owl:onClass <https://example.org/ccdh/CcdhString> ;
            owl:onProperty linkml:dysplasia_fraction ],
        [ a owl:Restriction ;
            owl:allValuesFrom <https://example.org/ccdh/Document> ;
            owl:onProperty linkml:related_document ],
        [ a owl:Restriction ;
            owl:maxQualifiedCardinality 1 ;
            owl:onClass <http://UNKNOWN.org/enum_CRDC-H.Specimen.specimen_type> ;
            owl:onProperty linkml:specimen_type ],
        [ a owl:Restriction ;
            owl:allValuesFrom <https://example.org/ccdh/Observation> ;
            owl:onProperty linkml:histological_composition_measure ],
        [ a owl:Restriction ;
            owl:maxQualifiedCardinality 1 ;
            owl:onClass <http://UNKNOWN.org/enum_CRDC-H.Specimen.morphlogy_assessment_method> ;
            owl:onProperty linkml:morphlogy_assessment_method ],
        [ a owl:Restriction ;
            owl:maxQualifiedCardinality 1 ;
            owl:onClass <http://UNKNOWN.org/enum_CRDC-H.Specimen.tumor_status_at_collection> ;
            owl:onProperty linkml:tumor_status_at_collection ],
        [ a owl:Restriction ;
            owl:maxQualifiedCardinality 1 ;
            owl:onClass <https://example.org/ccdh/Quantity> ;
            owl:onProperty linkml:distance_from_paired_specimen ],
        [ a owl:Restriction ;
            owl:allValuesFrom <https://example.org/ccdh/BiologicProduct> ;
            owl:onProperty linkml:derived_product ],
        [ a owl:Restriction ;
            owl:maxQualifiedCardinality 1 ;
            owl:onClass <https://example.org/ccdh/CcdhBoolean> ;
            owl:onProperty linkml:morphology_pathologically_confirmed ],
        [ a owl:Restriction ;
            owl:maxQualifiedCardinality 1 ;
            owl:onClass <http://UNKNOWN.org/enum_CRDC-H.Specimen.general_tissue_morphology> ;
            owl:onProperty linkml:general_tissue_morphology ],
        [ a owl:Restriction ;
            owl:maxQualifiedCardinality 1 ;
            owl:onClass <http://UNKNOWN.org/enum_CRDC-H.Specimen.morphology_assessor_role> ;
            owl:onProperty linkml:morphology_assessor_role ],
        [ a owl:Restriction ;
            owl:maxQualifiedCardinality 1 ;
            owl:onClass <https://example.org/ccdh/CcdhString> ;
            owl:onProperty linkml:id ],
        [ a owl:Restriction ;
            owl:allValuesFrom <https://example.org/ccdh/Specimen> ;
            owl:onProperty linkml:parent_specimen ],
        [ a owl:Restriction ;
            owl:allValuesFrom <https://example.org/ccdh/SpecimenProcessingActivity> ;
            owl:onProperty linkml:processing_activity ],
        [ a owl:Restriction ;
            owl:maxQualifiedCardinality 1 ;
            owl:onClass <https://example.org/ccdh/CcdhString> ;
            owl:onProperty linkml:description ],
        [ a owl:Restriction ;
            owl:maxQualifiedCardinality 1 ;
            owl:onClass <https://example.org/ccdh/SpecimenTransportActivity> ;
            owl:onProperty linkml:transport_activity ],
        [ a owl:Restriction ;
            owl:maxQualifiedCardinality 1 ;
            owl:onClass <http://UNKNOWN.org/enum_CRDC-H.Specimen.cellular_composition_type> ;
            owl:onProperty linkml:cellular_composition_type ],
        [ a owl:Restriction ;
            owl:allValuesFrom <https://example.org/ccdh/Observation> ;
            owl:onProperty linkml:quantity_measure ],
        [ a owl:Restriction ;
            owl:allValuesFrom <https://example.org/ccdh/Identifier> ;
            owl:onProperty linkml:identifier ],
        [ a owl:Restriction ;
            owl:maxQualifiedCardinality 1 ;
            owl:onClass <https://example.org/ccdh/Subject> ;
            owl:onProperty linkml:source_subject ],
        [ a owl:Restriction ;
            owl:maxQualifiedCardinality 1 ;
            owl:onClass <http://UNKNOWN.org/enum_CRDC-H.Specimen.specific_tissue_morphology> ;
            owl:onProperty linkml:specific_tissue_morphology ],
        [ a owl:Restriction ;
            owl:maxQualifiedCardinality 1 ;
            owl:onClass <https://example.org/ccdh/SpecimenStorageActivity> ;
            owl:onProperty linkml:storage_activity ],
        [ a owl:Restriction ;
            owl:maxQualifiedCardinality 1 ;
            owl:onClass <http://UNKNOWN.org/enum_CRDC-H.Specimen.preinvasive_tissue_morphology> ;
            owl:onProperty linkml:preinvasive_tissue_morphology ],
        <https://example.org/ccdh/Entity> ;
    skos:definition "Any material taken as a sample from a biological entity (living or dead), or from a physical object or the environment. Specimens are usually collected as an example of their kind, often for use in some investigation." ;
    skos:editorialNote "Derived from [Specimen in sheet Specimen](https://docs.google.com/spreadsheets/d/1oWS7cao-fgz2MKWtyr8h2dEL9unX__0bJrWKv6mQmM4/edit#gid=1439310281)" .

<https://example.org/ccdh/SpecimenContainer> a owl:Class,
        linkml:ClassDefinition ;
    rdfs:label "SpecimenContainer" ;
    rdfs:subClassOf [ a owl:Restriction ;
            owl:maxQualifiedCardinality 1 ;
            owl:onClass <http://UNKNOWN.org/enum_CRDC-H.SpecimenContainer.charge_type> ;
            owl:onProperty linkml:charge_type ],
        [ a owl:Restriction ;
            owl:allValuesFrom <https://example.org/ccdh/Substance> ;
            owl:onProperty linkml:additive ],
        [ a owl:Restriction ;
            owl:allValuesFrom <https://example.org/ccdh/SpecimenContainer> ;
            owl:onProperty linkml:parent_container ],
        [ a owl:Restriction ;
            owl:maxQualifiedCardinality 1 ;
            owl:onClass <https://example.org/ccdh/CcdhString> ;
            owl:onProperty linkml:id ],
        [ a owl:Restriction ;
            owl:maxQualifiedCardinality 1 ;
            owl:onClass <https://example.org/ccdh/CcdhString> ;
            owl:onProperty linkml:container_number ],
        [ a owl:Restriction ;
            owl:allValuesFrom <https://example.org/ccdh/Identifier> ;
            owl:onProperty linkml:identifier ],
        [ a owl:Restriction ;
            owl:maxQualifiedCardinality 1 ;
            owl:onClass <http://UNKNOWN.org/enum_CRDC-H.SpecimenContainer.container_type> ;
            owl:onProperty linkml:container_type ],
        <https://example.org/ccdh/Entity> ;
    skos:definition "A vessel in which a specimen is held or attached - to store or as a substrate for growth (e.g. a cell culture dish) or analysis (e.g. a microscope slide or 96-well plate)" ;
    skos:editorialNote "Derived from [SpecimenContainer in sheet SpecimenContainer](https://docs.google.com/spreadsheets/d/1oWS7cao-fgz2MKWtyr8h2dEL9unX__0bJrWKv6mQmM4/edit#gid=729222697)" .

<https://example.org/ccdh/BodySite> a owl:Class,
        linkml:ClassDefinition ;
    rdfs:label "BodySite" ;
    rdfs:subClassOf [ a owl:Restriction ;
            owl:allValuesFrom <http://UNKNOWN.org/enum_CRDC-H.BodySite.qualifier> ;
            owl:onProperty linkml:qualifier ],
        [ a owl:Restriction ;
            owl:onClass <http://UNKNOWN.org/enum_CRDC-H.BodySite.site> ;
            owl:onProperty linkml:site ;
            owl:qualifiedCardinality 1 ],
        <https://example.org/ccdh/Entity> ;
    skos:definition "" ;
    skos:editorialNote "Derived from [BodySite in sheet BodySite](https://docs.google.com/spreadsheets/d/1oWS7cao-fgz2MKWtyr8h2dEL9unX__0bJrWKv6mQmM4/edit#gid=1097478901)" .

<https://example.org/ccdh/Diagnosis> a owl:Class,
        linkml:ClassDefinition ;
    rdfs:label "Diagnosis" ;
    rdfs:subClassOf [ a owl:Restriction ;
            owl:maxQualifiedCardinality 1 ;
            owl:onClass <http://UNKNOWN.org/enum_CRDC-H.Diagnosis.morphology> ;
            owl:onProperty linkml:morphology ],
        [ a owl:Restriction ;
            owl:maxQualifiedCardinality 1 ;
            owl:onClass <https://example.org/ccdh/Quantity> ;
            owl:onProperty linkml:age_at_diagnosis ],
        [ a owl:Restriction ;
            owl:allValuesFrom <https://example.org/ccdh/BodySite> ;
            owl:onProperty linkml:primary_site ],
        [ a owl:Restriction ;
            owl:maxQualifiedCardinality 1 ;
            owl:onClass <https://example.org/ccdh/CcdhInteger> ;
            owl:onProperty linkml:year_at_diagnosis ],
        [ a owl:Restriction ;
            owl:allValuesFrom <https://example.org/ccdh/BodySite> ;
            owl:onProperty linkml:metastatic_site ],
        [ a owl:Restriction ;
            owl:maxQualifiedCardinality 1 ;
            owl:onClass <http://UNKNOWN.org/enum_CRDC-H.Diagnosis.condition> ;
            owl:onProperty linkml:condition ],
        [ a owl:Restriction ;
            owl:allValuesFrom <https://example.org/ccdh/Identifier> ;
            owl:onProperty linkml:identifier ],
        [ a owl:Restriction ;
            owl:maxQualifiedCardinality 1 ;
            owl:onClass <http://UNKNOWN.org/enum_CRDC-H.Diagnosis.disease_status> ;
            owl:onProperty linkml:disease_status ],
        [ a owl:Restriction ;
            owl:allValuesFrom <https://example.org/ccdh/Specimen> ;
            owl:onProperty linkml:related_specimen ],
        [ a owl:Restriction ;
            owl:maxQualifiedCardinality 1 ;
            owl:onClass <http://UNKNOWN.org/enum_CRDC-H.Diagnosis.method_of_diagnosis> ;
            owl:onProperty linkml:method_of_diagnosis ],
        [ a owl:Restriction ;
            owl:allValuesFrom <https://example.org/ccdh/CancerStageObservationSet> ;
            owl:onProperty linkml:stage ],
        [ a owl:Restriction ;
            owl:maxQualifiedCardinality 1 ;
            owl:onClass <https://example.org/ccdh/Diagnosis> ;
            owl:onProperty linkml:prior_diagnosis ],
        [ a owl:Restriction ;
            owl:allValuesFrom <https://example.org/ccdh/Entity> ;
            owl:onProperty linkml:grade ],
        [ a owl:Restriction ;
            owl:maxQualifiedCardinality 1 ;
            owl:onClass <https://example.org/ccdh/CcdhString> ;
            owl:onProperty linkml:id ],
        <https://example.org/ccdh/Entity> ;
    skos:definition "" ;
    skos:editorialNote "Derived from [Diagnosis in sheet Diagnosis](https://docs.google.com/spreadsheets/d/1oWS7cao-fgz2MKWtyr8h2dEL9unX__0bJrWKv6mQmM4/edit#gid=1015759209)" .

<https://example.org/ccdh/Subject> a owl:Class,
        linkml:ClassDefinition ;
    rdfs:label "Subject" ;
    rdfs:subClassOf [ a owl:Restriction ;
            owl:maxQualifiedCardinality 1 ;
            owl:onClass <http://UNKNOWN.org/enum_CRDC-H.Subject.vital_status> ;
            owl:onProperty linkml:vital_status ],
        [ a owl:Restriction ;
            owl:maxQualifiedCardinality 1 ;
            owl:onClass <http://UNKNOWN.org/enum_CRDC-H.Subject.ethnicity> ;
            owl:onProperty linkml:ethnicity ],
        [ a owl:Restriction ;
            owl:maxQualifiedCardinality 1 ;
            owl:onClass <http://UNKNOWN.org/enum_CRDC-H.Subject.species> ;
            owl:onProperty linkml:species ],
        [ a owl:Restriction ;
            owl:maxQualifiedCardinality 1 ;
            owl:onClass <http://UNKNOWN.org/enum_CRDC-H.Subject.cause_of_death> ;
            owl:onProperty linkml:cause_of_death ],
        [ a owl:Restriction ;
            owl:maxQualifiedCardinality 1 ;
            owl:onClass <http://UNKNOWN.org/enum_CRDC-H.Subject.breed> ;
            owl:onProperty linkml:breed ],
        [ a owl:Restriction ;
            owl:maxQualifiedCardinality 1 ;
            owl:onClass <http://UNKNOWN.org/enum_CRDC-H.Subject.sex> ;
            owl:onProperty linkml:sex ],
        [ a owl:Restriction ;
            owl:maxQualifiedCardinality 1 ;
            owl:onClass <https://example.org/ccdh/CcdhInteger> ;
            owl:onProperty linkml:year_of_death ],
        [ a owl:Restriction ;
            owl:allValuesFrom <http://UNKNOWN.org/enum_CRDC-H.Subject.race> ;
            owl:onProperty linkml:race ],
        [ a owl:Restriction ;
            owl:maxQualifiedCardinality 1 ;
            owl:onClass <https://example.org/ccdh/CcdhInteger> ;
            owl:onProperty linkml:year_of_birth ],
        [ a owl:Restriction ;
            owl:allValuesFrom <https://example.org/ccdh/Identifier> ;
            owl:onProperty linkml:identifier ],
        [ a owl:Restriction ;
            owl:onClass <https://example.org/ccdh/CcdhString> ;
            owl:onProperty linkml:id ;
            owl:qualifiedCardinality 1 ],
        [ a owl:Restriction ;
            owl:maxQualifiedCardinality 1 ;
            owl:onClass <https://example.org/ccdh/Quantity> ;
            owl:onProperty linkml:age_at_death ],
        <https://example.org/ccdh/Entity> ;
    skos:definition "Demographics and other administrative information about an individual or animal receiving care or other health-related services." ;
    skos:editorialNote "Derived from [Subject in sheet Subject](https://docs.google.com/spreadsheets/d/1oWS7cao-fgz2MKWtyr8h2dEL9unX__0bJrWKv6mQmM4/edit#gid=1651956379)" .

<https://example.org/ccdh/Substance> a owl:Class,
        linkml:ClassDefinition ;
    rdfs:label "Substance" ;
    rdfs:subClassOf [ a owl:Restriction ;
            owl:allValuesFrom <http://UNKNOWN.org/enum_CRDC-H.Substance.role> ;
            owl:onProperty linkml:role ],
        [ a owl:Restriction ;
            owl:maxQualifiedCardinality 1 ;
            owl:onClass <http://UNKNOWN.org/enum_CRDC-H.Substance.substance_type> ;
            owl:onProperty linkml:substance_type ],
        <https://example.org/ccdh/Entity> ;
    skos:definition "A type of material substance, or instance thereof,  as used in a particular application. May include information about the role the substance played in a particular application." ;
    skos:editorialNote "Derived from [Substance in sheet Substance](https://docs.google.com/spreadsheets/d/1oWS7cao-fgz2MKWtyr8h2dEL9unX__0bJrWKv6mQmM4/edit#gid=385534272)" .

<https://example.org/ccdh/CcdhInteger> a owl:Class,
        linkml:TypeDefinition ;
    rdfs:label "ccdh_integer" ;
    rdfs:subClassOf linkml:Integer ;
    skos:definition """An integer number.  This data type is based on the decimal type, but the fractional component is not allowed.  There are no restrictions on the size of the integer.
""" ;
    skos:editorialNote "Derived from [ccdh_integer in sheet Primitives](https://docs.google.com/spreadsheets/d/1oWS7cao-fgz2MKWtyr8h2dEL9unX__0bJrWKv6mQmM4/edit#gid=497370447)" .

<https://example.org/ccdh/Observation> a owl:Class,
        linkml:ClassDefinition ;
    rdfs:label "Observation" ;
    rdfs:subClassOf [ a owl:Restriction ;
            owl:maxQualifiedCardinality 1 ;
            owl:onClass <https://example.org/ccdh/Organization> ;
            owl:onProperty linkml:performed_by ],
        [ a owl:Restriction ;
            owl:maxQualifiedCardinality 1 ;
            owl:onClass <http://UNKNOWN.org/enum_CRDC-H.Observation.valueCodeableConcept> ;
            owl:onProperty linkml:valueCodeableConcept ],
        [ a owl:Restriction ;
            owl:maxQualifiedCardinality 1 ;
            owl:onClass <https://example.org/ccdh/CcdhDateTime> ;
            owl:onProperty linkml:valueDateTime ],
        [ a owl:Restriction ;
            owl:maxQualifiedCardinality 1 ;
            owl:onClass <https://example.org/ccdh/Entity> ;
            owl:onProperty linkml:valueEntity ],
        [ a owl:Restriction ;
            owl:allValuesFrom <http://UNKNOWN.org/enum_CRDC-H.Observation.method_type> ;
            owl:onProperty linkml:method_type ],
        [ a owl:Restriction ;
            owl:maxQualifiedCardinality 1 ;
            owl:onClass <https://example.org/ccdh/Quantity> ;
            owl:onProperty linkml:valueQuantity ],
        [ a owl:Restriction ;
            owl:maxQualifiedCardinality 1 ;
            owl:onClass <https://example.org/ccdh/Subject> ;
            owl:onProperty linkml:subject ],
        [ a owl:Restriction ;
            owl:maxQualifiedCardinality 1 ;
            owl:onClass <https://example.org/ccdh/CcdhString> ;
            owl:onProperty linkml:valueString ],
        [ a owl:Restriction ;
            owl:allValuesFrom <https://example.org/ccdh/Entity> ;
            owl:onProperty linkml:focus ],
        [ a owl:Restriction ;
            owl:onClass <https://example.org/ccdh/CcdhString> ;
            owl:onProperty linkml:id ;
            owl:qualifiedCardinality 1 ],
        [ a owl:Restriction ;
            owl:onClass <http://UNKNOWN.org/enum_CRDC-H.Observation.observation_type> ;
            owl:onProperty linkml:observation_type ;
            owl:qualifiedCardinality 1 ],
        [ a owl:Restriction ;
            owl:maxQualifiedCardinality 1 ;
            owl:onClass <https://example.org/ccdh/CcdhBoolean> ;
            owl:onProperty linkml:valueBoolean ],
        [ a owl:Restriction ;
            owl:onClass <http://UNKNOWN.org/enum_CRDC-H.Observation.category> ;
            owl:onProperty linkml:category ;
            owl:qualifiedCardinality 1 ],
        [ a owl:Restriction ;
            owl:maxQualifiedCardinality 1 ;
            owl:onClass <https://example.org/ccdh/CcdhDecimal> ;
            owl:onProperty linkml:valueDecimal ],
        [ a owl:Restriction ;
            owl:maxQualifiedCardinality 1 ;
            owl:onClass <https://example.org/ccdh/CcdhDecimal> ;
            owl:onProperty linkml:valueInteger ],
        <https://example.org/ccdh/Entity> ;
    skos:definition "A structured object that describes a single data item about an entity, as generated through a point-in-time observation, measurement, or interpretation." ;
    skos:editorialNote "Derived from [Observation in sheet Observation](https://docs.google.com/spreadsheets/d/1oWS7cao-fgz2MKWtyr8h2dEL9unX__0bJrWKv6mQmM4/edit#gid=550424063)" .

<https://example.org/ccdh/CcdhDateTime> a owl:Class,
        linkml:TypeDefinition ;
    rdfs:label "ccdh_dateTime" ;
    rdfs:subClassOf linkml:Datetime ;
    skos:definition "A date and time string specified using a specialized concatenation of the date and time data types, in the general format YYYY-MM-DDThh:mm:ss+zz:zz.  " ;
    skos:editorialNote "Derived from [ccdh_dateTime in sheet Primitives](https://docs.google.com/spreadsheets/d/1oWS7cao-fgz2MKWtyr8h2dEL9unX__0bJrWKv6mQmM4/edit#gid=497370447)" .

linkml:topValue a owl:DatatypeProperty ;
    rdfs:label "value" .

<https://example.org/ccdh/Quantity> a owl:Class,
        linkml:ClassDefinition ;
    rdfs:label "Quantity" ;
    rdfs:subClassOf [ a owl:Restriction ;
            owl:maxQualifiedCardinality 1 ;
            owl:onClass <https://example.org/ccdh/CcdhString> ;
            owl:onProperty linkml:unit ],
        [ a owl:Restriction ;
            owl:maxQualifiedCardinality 1 ;
            owl:onClass <https://example.org/ccdh/CcdhDecimal> ;
            owl:onProperty linkml:valueDecimal ],
        [ a owl:Restriction ;
            owl:maxQualifiedCardinality 1 ;
            owl:onClass <https://example.org/ccdh/Coding> ;
            owl:onProperty linkml:comparator ],
        [ a owl:Restriction ;
            owl:maxQualifiedCardinality 1 ;
            owl:onClass <http://UNKNOWN.org/enum_CRDC-H.Quantity.valueCodeableConcept> ;
            owl:onProperty linkml:valueCodeableConcept ],
        [ a owl:Restriction ;
            owl:maxQualifiedCardinality 1 ;
            owl:onClass <https://example.org/ccdh/Coding> ;
            owl:onProperty linkml:unitCode ],
        <https://example.org/ccdh/Entity> ;
    skos:definition "A structured object to represent an amount of something (e.g., weight, mass, length, duration of time) - including a value and unit." ;
    skos:editorialNote "Derived from [Quantity in sheet Quantity](https://docs.google.com/spreadsheets/d/1oWS7cao-fgz2MKWtyr8h2dEL9unX__0bJrWKv6mQmM4/edit#gid=1941950611)" .

<https://example.org/ccdh/Organization> a owl:Class,
        linkml:ClassDefinition ;
    rdfs:label "Organization" ;
    rdfs:subClassOf [ a owl:Restriction ;
            owl:maxQualifiedCardinality 1 ;
            owl:onClass <https://example.org/ccdh/CcdhString> ;
            owl:onProperty linkml:name ],
        [ a owl:Restriction ;
            owl:maxQualifiedCardinality 1 ;
            owl:onClass <https://example.org/ccdh/CcdhString> ;
            owl:onProperty linkml:alias ],
        [ a owl:Restriction ;
            owl:maxQualifiedCardinality 1 ;
            owl:onClass <https://example.org/ccdh/CcdhString> ;
            owl:onProperty linkml:organization_type ],
        [ a owl:Restriction ;
            owl:allValuesFrom <https://example.org/ccdh/Identifier> ;
            owl:onProperty linkml:identifier ],
        [ a owl:Restriction ;
            owl:onClass <https://example.org/ccdh/CcdhString> ;
            owl:onProperty linkml:id ;
            owl:qualifiedCardinality 1 ],
        <https://example.org/ccdh/Entity> ;
    skos:definition "A grouping of people or organizations with a common purpose such as a data coordinating center, an university, or an institute within a university" ;
    skos:editorialNote "Derived from [Organization in sheet Organization](https://docs.google.com/spreadsheets/d/1oWS7cao-fgz2MKWtyr8h2dEL9unX__0bJrWKv6mQmM4/edit#gid=1477577710)" .

linkml:TypeDefinition a owl:Class ;
    rdfs:label "type_definition" ;
    skos:definition "A data type definition." .

<https://example.org/ccdh/Identifier> a owl:Class,
        linkml:ClassDefinition ;
    rdfs:label "Identifier" ;
    rdfs:subClassOf [ a owl:Restriction ;
            owl:onClass <https://example.org/ccdh/CcdhString> ;
            owl:onProperty linkml:value ;
            owl:qualifiedCardinality 1 ],
        [ a owl:Restriction ;
            owl:maxQualifiedCardinality 1 ;
            owl:onClass <https://example.org/ccdh/CcdhString> ;
            owl:onProperty linkml:system ],
        [ a owl:Restriction ;
            owl:maxQualifiedCardinality 1 ;
            owl:onClass <http://UNKNOWN.org/enum_CRDC-H.Identifier.type> ;
            owl:onProperty linkml:type ],
        <https://example.org/ccdh/Entity> ;
    skos:definition "An Identifier is associated with a unique object or entity within a given system." ;
    skos:editorialNote "Derived from [Identifier in sheet Identifier](https://docs.google.com/spreadsheets/d/1oWS7cao-fgz2MKWtyr8h2dEL9unX__0bJrWKv6mQmM4/edit#gid=1307792462)" .

<https://example.org/ccdh/TimePoint> a owl:Class,
        linkml:ClassDefinition ;
    rdfs:label "TimePoint" ;
    rdfs:subClassOf [ a owl:Restriction ;
            owl:maxQualifiedCardinality 1 ;
            owl:onClass <http://UNKNOWN.org/enum_CRDC-H.TimePoint.indexEventType> ;
            owl:onProperty linkml:indexEventType ],
        [ a owl:Restriction ;
            owl:maxQualifiedCardinality 1 ;
            owl:onClass <https://example.org/ccdh/CcdhDateTime> ;
            owl:onProperty linkml:indexDate ],
        [ a owl:Restriction ;
            owl:maxQualifiedCardinality 1 ;
            owl:onClass <https://example.org/ccdh/Quantity> ;
            owl:onProperty linkml:offsetFromIndex ],
        [ a owl:Restriction ;
            owl:maxQualifiedCardinality 1 ;
            owl:onClass <https://example.org/ccdh/CcdhDateTime> ;
            owl:onProperty linkml:dateTime ],
        <https://example.org/ccdh/Entity> ;
    skos:definition "A structured representation of a single point in time that allows direct/explicit declaration as a dateTime, or specification in terms of offset from a defiend index." ;
    skos:editorialNote "Derived from [TimePoint in sheet TimePoint](https://docs.google.com/spreadsheets/d/1oWS7cao-fgz2MKWtyr8h2dEL9unX__0bJrWKv6mQmM4/edit#gid=300932847)" .

linkml:ClassDefinition a owl:Class ;
    rdfs:label "class_definition" ;
    skos:definition "the definition of a class or interface" .

<https://example.org/ccdh/Entity> a owl:Class,
        linkml:ClassDefinition ;
    rdfs:label "Entity" ;
    rdfs:subClassOf [ a owl:Restriction ;
            owl:maxQualifiedCardinality 1 ;
            owl:onClass <https://example.org/ccdh/CcdhString> ;
            owl:onProperty linkml:id ] ;
    skos:definition "Any resource that has its own identifier" ;
    skos:editorialNote "Derived from [Entity in sheet Entity](https://docs.google.com/spreadsheets/d/1oWS7cao-fgz2MKWtyr8h2dEL9unX__0bJrWKv6mQmM4/edit#gid=65213867)" .

<https://example.org/ccdh/CcdhString> a owl:Class,
        linkml:TypeDefinition ;
    rdfs:label "ccdh_string" ;
    rdfs:subClassOf linkml:String ;
    skos:definition "A sequence of Unicode characters.  There are no limits on the number of characters in the string." ;
    skos:editorialNote "Derived from [ccdh_string in sheet Primitives](https://docs.google.com/spreadsheets/d/1oWS7cao-fgz2MKWtyr8h2dEL9unX__0bJrWKv6mQmM4/edit#gid=497370447)" .

linkml:SlotDefinition a owl:Class ;
    rdfs:label "slot_definition" ;
    skos:definition "the definition of a property or a slot" .



